Tuned

Simple_Prover/Simple_Prover.thy
@@ -1,526 +1,528 @@
 (* Authors: Jørgen Villadsen, Anders Schlichtkrull, Andreas Halkjær From *)
 
-section "A Certified Simple Prover for First-Order Logic"
+section \<open>A Certified Simple Prover for First-Order Logic\<close>
 
 theory Simple_Prover imports Main begin
 
-section "Syntax and Semantics"
+section \<open>Preliminaries\<close>
+
+primrec dec :: \<open>nat \<Rightarrow> nat\<close> where
+  \<open>dec 0 = 0\<close> |
+  \<open>dec (Suc n) = n\<close>
+
+primrec sub :: \<open>nat \<Rightarrow> nat \<Rightarrow> nat\<close> where
+  \<open>sub x 0 = x\<close> |
+  \<open>sub x (Suc n) = dec (sub x n)\<close>
+
+primrec add :: \<open>nat \<Rightarrow> nat \<Rightarrow> nat\<close> where
+  \<open>add x 0 = x\<close> |
+  \<open>add x (Suc n) = Suc (add x n)\<close>
+
+lemma append_simps: \<open>[] @ l = l\<close> \<open>(h # t) @ l = h # t @ l\<close>
+  by (rule append.simps(1),rule append.simps(2))
+
+lemma if_simps: \<open>(if True then x else y) = x\<close> \<open>(if False then x else y) = y\<close>
+  by (rule if_True,rule if_False)
+
+lemma not_simps: \<open>(\<not> True) = False\<close> \<open>(\<not> False) = True\<close>
+  by (rule not_True_eq_False,rule not_False_eq_True)
+
+lemma prod_simps: \<open>fst (x,y) = x\<close> \<open>snd (x,y) = y\<close>
+  unfolding fst_def snd_def
+  by (rule prod.case,rule prod.case)
+
+lemma nat_simps: \<open>(0 = 0) = True\<close>
+  by (rule simp_thms)
+
+lemma list_simps: \<open>([] = []) = True\<close>
+  by (rule simp_thms)
+
+lemma bool_simps: \<open>(True = True) = True\<close> \<open>(False = False) = True\<close>
+  by (rule simp_thms,rule simp_thms)
+
+lemma inject_simps: \<open>(True \<and> b) = b\<close> \<open>(False \<and> b) = False\<close>
+  by (rule simp_thms,rule simp_thms)
+
+section \<open>Syntax and Semantics\<close>
 
 type_synonym id = nat
 
-datatype nnf = Pre bool id "nat list" | Con nnf nnf | Dis nnf nnf | Uni nnf | Exi nnf
+datatype nnf = Pre bool id \<open>nat list\<close> | Con nnf nnf | Dis nnf nnf | Uni nnf | Exi nnf
 
-abbreviation (input) "TEST P Q \<equiv> (\<exists>x. P x \<or> Q x) \<longrightarrow> (\<exists>x. Q x) \<or> (\<exists>x. P x)"
+abbreviation (input) \<open>TEST P Q \<equiv> (\<exists>x. P x \<or> Q x) \<longrightarrow> (\<exists>x. Q x) \<or> (\<exists>x. P x)\<close>
 
-proposition "TEST P Q"
-by iprover
+proposition \<open>TEST P Q\<close>
+  by iprover
 
-proposition "TEST P Q = (\<forall>x. \<not> P x \<and> \<not> Q x) \<or> (\<exists>x. Q x) \<or> (\<exists>x. P x)"
-by fast
+proposition \<open>TEST P Q = (\<forall>x. \<not> P x \<and> \<not> Q x) \<or> (\<exists>x. Q x) \<or> (\<exists>x. P x)\<close>
+  by fast
 
-abbreviation (input) "P_id \<equiv> 0"
+abbreviation (input) \<open>P_id \<equiv> 0\<close>
 
-abbreviation (input) "Q_id \<equiv> Suc 0"
+abbreviation (input) \<open>Q_id \<equiv> Suc 0\<close>
 
-definition \<comment> "TEST P Q"
-  "test \<equiv> Dis
+definition \<comment> \<open>TEST P Q\<close>
+  \<open>test \<equiv> Dis
     (Uni (Con (Pre False P_id [0]) (Pre False Q_id [0])))
-    (Dis (Exi (Pre True Q_id [0])) (Exi (Pre True P_id [0])))"
+    (Dis (Exi (Pre True Q_id [0])) (Exi (Pre True P_id [0])))\<close>
 
-type_synonym proxy = "unit list"
+type_synonym proxy = \<open>unit list\<close>
 
-type_synonym model = "proxy set \<times> (id \<Rightarrow> proxy list \<Rightarrow> bool)"
+type_synonym model = \<open>proxy set \<times> (id \<Rightarrow> proxy list \<Rightarrow> bool)\<close>
 
-type_synonym environment = "nat \<Rightarrow> proxy"
+type_synonym environment = \<open>nat \<Rightarrow> proxy\<close>
 
-definition is_model_environment :: "model \<Rightarrow> environment \<Rightarrow> bool" where
-  "is_model_environment m e \<equiv> \<forall>n. e n \<in> fst m"
+definition is_model_environment :: \<open>model \<Rightarrow> environment \<Rightarrow> bool\<close> where
+  \<open>is_model_environment m e \<equiv> \<forall>n. e n \<in> fst m\<close>
 
-primrec semantics :: "model \<Rightarrow> environment \<Rightarrow> nnf \<Rightarrow> bool" where
-  "semantics m e (Pre b i v) = (b = snd m i (map e v))" |
-  "semantics m e (Con p q) = (semantics m e p \<and> semantics m e q)" |
-  "semantics m e (Dis p q) = (semantics m e p \<or> semantics m e q)" |
-  "semantics m e (Uni p) = (\<forall>z \<in> fst m. semantics m (\<lambda>x. case x of 0 \<Rightarrow> z | Suc n \<Rightarrow> e n) p)" |
-  "semantics m e (Exi p) = (\<exists>z \<in> fst m. semantics m (\<lambda>x. case x of 0 \<Rightarrow> z | Suc n \<Rightarrow> e n) p)"
+primrec semantics :: \<open>model \<Rightarrow> environment \<Rightarrow> nnf \<Rightarrow> bool\<close> where
+  \<open>semantics m e (Pre b i v) = (b = snd m i (map e v))\<close> |
+  \<open>semantics m e (Con p q) = (semantics m e p \<and> semantics m e q)\<close> |
+  \<open>semantics m e (Dis p q) = (semantics m e p \<or> semantics m e q)\<close> |
+  \<open>semantics m e (Uni p) = (\<forall>z \<in> fst m. semantics m (\<lambda>x. case x of 0 \<Rightarrow> z | Suc n \<Rightarrow> e n) p)\<close> |
+  \<open>semantics m e (Exi p) = (\<exists>z \<in> fst m. semantics m (\<lambda>x. case x of 0 \<Rightarrow> z | Suc n \<Rightarrow> e n) p)\<close>
 
-section "Sequent Calculus"
+section \<open>Sequent Calculus\<close>
 
-primrec dash :: "nat list \<Rightarrow> nat \<Rightarrow> nat list" where
-  "dash l 0 = l" |
-  "dash l (Suc n) = n # l"
+primrec dash :: \<open>nat list \<Rightarrow> nat \<Rightarrow> nat list\<close> where
+  \<open>dash l 0 = l\<close> |
+  \<open>dash l (Suc n) = n # l\<close>
 
-primrec dump :: "nat list \<Rightarrow> nat list" where
-  "dump [] = []" |
-  "dump (h # t) = dash (dump t) h"
+primrec dump :: \<open>nat list \<Rightarrow> nat list\<close> where
+  \<open>dump [] = []\<close> |
+  \<open>dump (h # t) = dash (dump t) h\<close>
 
-primrec free :: "nnf \<Rightarrow> nat list" where
-  "free (Pre _ _ v) = v" |
-  "free (Con p q) = free p @ free q" |
-  "free (Dis p q) = free p @ free q" |
-  "free (Uni p) = dump (free p)" |
-  "free (Exi p) = dump (free p)"
+primrec free :: \<open>nnf \<Rightarrow> nat list\<close> where
+  \<open>free (Pre _ _ v) = v\<close> |
+  \<open>free (Con p q) = free p @ free q\<close> |
+  \<open>free (Dis p q) = free p @ free q\<close> |
+  \<open>free (Uni p) = dump (free p)\<close> |
+  \<open>free (Exi p) = dump (free p)\<close>
 
-primrec frees :: "nnf list \<Rightarrow> nat list" where
-  "frees [] = []" |
-  "frees (h # t) = free h @ frees t"
+primrec frees :: \<open>nnf list \<Rightarrow> nat list\<close> where
+  \<open>frees [] = []\<close> |
+  \<open>frees (h # t) = free h @ frees t\<close>
 
-primrec dec :: "nat \<Rightarrow> nat" where
-  "dec 0 = 0" |
-  "dec (Suc n) = n"
+primrec fresh :: \<open>nat list \<Rightarrow> nat\<close> where
+  \<open>fresh [] = 0\<close> |
+  \<open>fresh (h # t) = Suc (add (sub (dec (fresh t)) h) h)\<close>
 
-primrec sub :: "nat \<Rightarrow> nat \<Rightarrow> nat" where
-  "sub x 0 = x" |
-  "sub x (Suc n) = dec (sub x n)"
+primrec over :: \<open>nat \<Rightarrow> nat \<Rightarrow> nat \<Rightarrow> nat\<close> where
+  \<open>over s _ 0 = s\<close> |
+  \<open>over _ h (Suc _) = h\<close>
 
-primrec add :: "nat \<Rightarrow> nat \<Rightarrow> nat" where
-  "add x 0 = x" |
-  "add x (Suc n) = Suc (add x n)"
+primrec more :: \<open>nat \<Rightarrow> nat \<Rightarrow> nat \<Rightarrow> nat \<Rightarrow> nat\<close> where
+  \<open>more x s h 0 = over s h (sub x h)\<close> |
+  \<open>more _ _ h (Suc _) = dec h\<close>
 
-primrec fresh :: "nat list \<Rightarrow> nat" where
-  "fresh [] = 0" |
-  "fresh (h # t) = Suc (add (sub (dec (fresh t)) h) h)"
+primrec mend :: \<open>nat \<Rightarrow> nat \<Rightarrow> nat list \<Rightarrow> nat list\<close> where
+  \<open>mend _ _ [] = []\<close> |
+  \<open>mend x s (h # t) = more x s h (sub h x) # mend x s t\<close>
 
-primrec over :: "nat \<Rightarrow> nat \<Rightarrow> nat \<Rightarrow> nat" where
-  "over s _ 0 = s" |
-  "over _ h (Suc _) = h"
+primrec subst :: \<open>nat \<Rightarrow> nat \<Rightarrow> nnf \<Rightarrow> nnf\<close> where
+  \<open>subst x s (Pre b i v) = Pre b i (mend x s v)\<close> |
+  \<open>subst x s (Con p q) = Con (subst x s p) (subst x s q)\<close> |
+  \<open>subst x s (Dis p q) = Dis (subst x s p) (subst x s q)\<close> |
+  \<open>subst x s (Uni p) = Uni (subst (Suc x) (Suc s) p)\<close> |
+  \<open>subst x s (Exi p) = Exi (subst (Suc x) (Suc s) p)\<close>
 
-primrec more :: "nat \<Rightarrow> nat \<Rightarrow> nat \<Rightarrow> nat \<Rightarrow> nat" where
-  "more x s h 0 = over s h (sub x h)" |
-  "more _ _ h (Suc _) = dec h"
+type_synonym sequent = \<open>(nat \<times> nnf) list\<close>
 
-primrec mend :: "nat \<Rightarrow> nat \<Rightarrow> nat list \<Rightarrow> nat list" where
-  "mend _ _ [] = []" |
-  "mend x s (h # t) = more x s h (sub h x) # mend x s t"
+primrec base :: \<open>sequent \<Rightarrow> nnf list\<close> where
+  \<open>base [] = []\<close> |
+  \<open>base (h # t) = snd h # base t\<close>
 
-primrec subst :: "nat \<Rightarrow> nat \<Rightarrow> nnf \<Rightarrow> nnf" where
-  "subst x s (Pre b i v) = Pre b i (mend x s v)" |
-  "subst x s (Con p q) = Con (subst x s p) (subst x s q)" |
-  "subst x s (Dis p q) = Dis (subst x s p) (subst x s q)" |
-  "subst x s (Uni p) = Uni (subst (Suc x) (Suc s) p)" |
-  "subst x s (Exi p) = Exi (subst (Suc x) (Suc s) p)"
+primrec stop :: \<open>sequent list \<Rightarrow> nnf \<Rightarrow> nnf list \<Rightarrow> sequent list\<close> where
+  \<open>stop c _ [] = c\<close> |
+  \<open>stop c p (h # t) = (if p = h then [] else stop c p t)\<close>
 
-type_synonym sequent = "(nat \<times> nnf) list"
+primrec track :: \<open>sequent \<Rightarrow> nat \<Rightarrow> nnf \<Rightarrow> sequent list\<close> where
+  \<open>track s _ (Pre b i v) = stop [s @ [(0,Pre b i v)]] (Pre (\<not> b) i v) (base s)\<close> |
+  \<open>track s _ (Con p q) = [s @ [(0,p)],s @ [(0,q)]]\<close> |
+  \<open>track s _ (Dis p q) = [s @ [(0,p),(0,q)]]\<close> |
+  \<open>track s _ (Uni p) = [s @ [(0,subst 0 (fresh (frees (Uni p # base s))) p)]]\<close> |
+  \<open>track s n (Exi p) = [s @ [(0,subst 0 n p),(Suc n,Exi p)]]\<close>
 
-primrec base :: "sequent \<Rightarrow> nnf list" where
-  "base [] = []" |
-  "base (h # t) = snd h # base t"
+primrec solve :: \<open>sequent \<Rightarrow> sequent list\<close> where
+  \<open>solve [] = [[]]\<close> |
+  \<open>solve (h # t) = track t (fst h) (snd h)\<close>
 
-primrec stop :: "sequent list \<Rightarrow> nnf \<Rightarrow> nnf list \<Rightarrow> sequent list" where
-  "stop c _ [] = c" |
-  "stop c p (h # t) = (if p = h then [] else stop c p t)"
+primrec solves :: \<open>sequent list \<Rightarrow> sequent list\<close> where
+  \<open>solves [] = []\<close> |
+  \<open>solves (h # t) = solve h @ solves t\<close>
 
-primrec track :: "sequent \<Rightarrow> nat \<Rightarrow> nnf \<Rightarrow> sequent list" where
-  "track s _ (Pre b i v) = stop [s @ [(0,Pre b i v)]] (Pre (\<not> b) i v) (base s)" |
-  "track s _ (Con p q) = [s @ [(0,p)],s @ [(0,q)]]" |
-  "track s _ (Dis p q) = [s @ [(0,p),(0,q)]]" |
-  "track s _ (Uni p) = [s @ [(0,subst 0 (fresh (frees (Uni p # base s))) p)]]" |
-  "track s n (Exi p) = [s @ [(0,subst 0 n p),(Suc n,Exi p)]]"
+type_synonym 'a algorithm = \<open>('a \<Rightarrow> bool) \<Rightarrow> ('a \<Rightarrow> 'a) \<Rightarrow> 'a \<Rightarrow> bool\<close>
 
-primrec solve :: "sequent \<Rightarrow> sequent list" where
-  "solve [] = [[]]" |
-  "solve (h # t) = track t (fst h) (snd h)"
+primrec null :: \<open>'a list \<Rightarrow> bool\<close> where
+  \<open>null [] = True\<close> |
+  \<open>null (_ # _) = False\<close>
 
-primrec solves :: "sequent list \<Rightarrow> sequent list" where
-  "solves [] = []" |
-  "solves (h # t) = solve h @ solves t"
+definition main :: \<open>sequent list algorithm \<Rightarrow> nnf \<Rightarrow> bool\<close> where
+  \<open>main a p \<equiv> a null solves [[(0,p)]]\<close>
 
-type_synonym 'a algorithm = "('a \<Rightarrow> bool) \<Rightarrow> ('a \<Rightarrow> 'a) \<Rightarrow> 'a \<Rightarrow> bool"
+primrec repeat :: \<open>('a \<Rightarrow> 'a) \<Rightarrow> 'a \<Rightarrow> nat \<Rightarrow> 'a\<close> where
+  \<open>repeat _ c 0 = c\<close> |
+  \<open>repeat f c (Suc n) = repeat f (f c) n\<close>
 
-primrec null :: "'a list \<Rightarrow> bool" where
-  "null [] = True" |
-  "null (_ # _) = False"
+definition iterator :: \<open>'a algorithm\<close> where
+  \<open>iterator g f c \<equiv> \<exists>n. g (repeat f c n)\<close>
 
-definition main :: "sequent list algorithm \<Rightarrow> nnf \<Rightarrow> bool" where
-  "main a p \<equiv> a null solves [[(0,p)]]"
+definition check :: \<open>nnf \<Rightarrow> bool\<close> where
+  \<open>check \<equiv> main iterator\<close>
 
-primrec repeat :: "('a \<Rightarrow> 'a) \<Rightarrow> 'a \<Rightarrow> nat \<Rightarrow> 'a" where
-  "repeat _ c 0 = c" |
-  "repeat f c (Suc n) = repeat f (f c) n"
+section \<open>Prover\<close>
 
-definition iterator :: "'a algorithm" where
-  "iterator g f c \<equiv> \<exists>n. g (repeat f c n)"
+abbreviation (input) \<open>CHECK \<equiv> check = (\<lambda>p. \<forall>m e. is_model_environment m e \<longrightarrow> semantics m e p)\<close>
 
-definition check :: "nnf \<Rightarrow> bool" where
-  "check \<equiv> main iterator"
+abbreviation \<open>prover \<equiv> iterator null solves\<close>
 
-section "Prover"
+lemma check_prover: \<open>check p \<equiv> prover [[(0,p)]]\<close>
+  unfolding check_def main_def .
 
-abbreviation (input) "CHECK \<equiv> check = (\<lambda>p. \<forall>m e. is_model_environment m e \<longrightarrow> semantics m e p)"
+lemma iterator[code]: \<open>iterator g f c = (if g c then True else iterator g f (f c))\<close>
+  unfolding iterator_def
+  using repeat.simps not0_implies_Suc
+  by metis
 
-abbreviation "prover \<equiv> iterator null solves"
+lemma prover: \<open>prover c = (if null c then True else prover (solves c))\<close>
+  using iterator .
 
-lemma check_prover: "check p \<equiv> prover [[(0,p)]]"
-unfolding check_def main_def .
+lemma prover_next: \<open>prover (h # t) = prover (solves (h # t))\<close>
+  using prover
+  by simp
 
-lemma iterator[code]: "iterator g f c = (if g c then True else iterator g f (f c))"
-unfolding iterator_def
-using repeat.simps not0_implies_Suc
-by metis
-
-lemma prover: "prover c = (if null c then True else prover (solves c))"
-using iterator .
-
-lemma prover_next: "prover (h # t) = prover (solves (h # t))"
-using prover
-by simp
-
-lemma prover_done: "prover [] = True"
-using prover
-by simp
-
-lemma append_simps: "[] @ l = l" "(h # t) @ l = h # t @ l"
-by (rule append.simps(1),rule append.simps(2))
-
-lemma if_simps: "(if True then x else y) = x" "(if False then x else y) = y"
-by (rule if_True,rule if_False)
-
-lemma not_simps: "(\<not> True) = False" "(\<not> False) = True"
-by (rule not_True_eq_False,rule not_False_eq_True)
-
-lemma prod_simps: "fst (x,y) = x" "snd (x,y) = y"
-unfolding fst_def snd_def
-by (rule prod.case,rule prod.case)
-
-lemma nat_simps: "(0 = 0) = True"
-by (rule simp_thms)
-
-lemma list_simps: "([] = []) = True"
-by (rule simp_thms)
-
-lemma bool_simps: "(True = True) = True" "(False = False) = True"
-by (rule simp_thms,rule simp_thms)
-
-lemma inject_simps: "(True \<and> b) = b" "(False \<and> b) = False"
-by (rule simp_thms,rule simp_thms)
+lemma prover_done: \<open>prover [] = True\<close>
+  using prover
+  by simp
 
 lemmas simps = check_prover prover_next prover_done solves.simps solve.simps track.simps stop.simps
-  base.simps subst.simps mend.simps more.simps over.simps fresh.simps add.simps sub.simps
-  dec.simps frees.simps free.simps dump.simps dash.simps nnf.distinct nnf.inject append_simps
-  if_simps not_simps prod_simps nat.distinct list.distinct bool.distinct nat_simps list_simps
-  bool_simps prod.inject nat.inject list.inject inject_simps
+  base.simps subst.simps mend.simps more.simps over.simps fresh.simps frees.simps free.simps
+  dump.simps dash.simps nnf.distinct nnf.inject add.simps sub.simps dec.simps append_simps if_simps
+  not_simps prod_simps nat_simps list_simps bool_simps inject_simps nat.distinct list.distinct
+  bool.distinct prod.inject nat.inject list.inject
 
 theorem program:
-  "\<And>p. check p \<equiv> prover [[(0,p)]]"
-  "\<And>h t. prover (h # t) \<equiv> prover (solves (h # t))"
-  "prover [] \<equiv> True"
-  "solves [] \<equiv> []"
-  "\<And>h t. solves (h # t) \<equiv> solve h @ solves t"
-  "solve [] \<equiv> [[]]"
-  "\<And>h t. solve (h # t) \<equiv> track t (fst h) (snd h)"
-  "\<And>s n b i v. track s n (Pre b i v) \<equiv> stop [s @ [(0,Pre b i v)]] (Pre (\<not> b) i v) (base s)"
-  "\<And>s n p q. track s n (Con p q) \<equiv> [s @ [(0,p)],s @ [(0,q)]]"
-  "\<And>s n p q. track s n (Dis p q) \<equiv> [s @ [(0,p),(0,q)]]"
-  "\<And>s n p. track s n (Uni p) \<equiv> [s @ [(0,subst 0 (fresh (frees (Uni p # base s))) p)]]"
-  "\<And>s n p. track s n (Exi p) \<equiv> [s @ [(0,subst 0 n p),(Suc n,Exi p)]]"
-  "\<And>c p. stop c p [] \<equiv> c"
-  "\<And>c p h t. stop c p (h # t) \<equiv> (if p = h then [] else stop c p t)"
-  "base [] \<equiv> []"
-  "\<And>h t. base (h # t) \<equiv> snd h # base t"
-  "\<And>x s b i v. subst x s (Pre b i v) \<equiv> Pre b i (mend x s v)"
-  "\<And>x s p q. subst x s (Con p q) \<equiv> Con (subst x s p) (subst x s q)"
-  "\<And>x s p q. subst x s (Dis p q) \<equiv> Dis (subst x s p) (subst x s q)"
-  "\<And>x s p. subst x s (Uni p) \<equiv> Uni (subst (Suc x) (Suc s) p)"
-  "\<And>x s p. subst x s (Exi p) \<equiv> Exi (subst (Suc x) (Suc s) p)"
-  "\<And>x s. mend x s [] \<equiv> []"
-  "\<And>x s h t. mend x s (h # t) \<equiv> more x s h (sub h x) # mend x s t"
-  "\<And>x s h. more x s h 0 \<equiv> over s h (sub x h)"
-  "\<And>x s h n. more x s h (Suc n) \<equiv> dec h"
-  "\<And>s h. over s h 0 \<equiv> s"
-  "\<And>s h n. over s h (Suc n) \<equiv> h"
-  "fresh [] \<equiv> 0"
-  "\<And>h t. fresh (h # t) \<equiv> Suc (add (sub (dec (fresh t)) h) h)"
-  "\<And>x. add x 0 \<equiv> x"
-  "\<And>x n. add x (Suc n) \<equiv> Suc (add x n)"
-  "\<And>x. sub x 0 \<equiv> x"
-  "\<And>x n. sub x (Suc n) \<equiv> dec (sub x n)"
-  "dec 0 \<equiv> 0"
-  "\<And>n. dec (Suc n) \<equiv> n"
-  "frees [] \<equiv> []"
-  "\<And>h t. frees (h # t) \<equiv> free h @ frees t"
-  "\<And>b i v. free (Pre b i v) \<equiv> v"
-  "\<And>p q. free (Con p q) \<equiv> free p @ free q"
-  "\<And>p q. free (Dis p q) \<equiv> free p @ free q"
-  "\<And>p. free (Uni p) \<equiv> dump (free p)"
-  "\<And>p. free (Exi p) \<equiv> dump (free p)"
-  "dump [] \<equiv> []"
-  "\<And>h t. dump (h # t) \<equiv> dash (dump t) h"
-  "\<And>l. dash l 0 \<equiv> l"
-  "\<And>l n. dash l (Suc n) \<equiv> n # l"
-by ((simp only: simps(1)),
-    (simp only: simps(2)),
-    (simp only: simps(3)),
-    (simp only: simps(4)),
-    (simp only: simps(5)),
-    (simp only: simps(6)),
-    (simp only: simps(7)),
-    (simp only: simps(8)),
-    (simp only: simps(9)),
-    (simp only: simps(10)),
-    (simp only: simps(11)),
-    (simp only: simps(12)),
-    (simp only: simps(13)),
-    (simp only: simps(14)),
-    (simp only: simps(15)),
-    (simp only: simps(16)),
-    (simp only: simps(17)),
-    (simp only: simps(18)),
-    (simp only: simps(19)),
-    (simp only: simps(20)),
-    (simp only: simps(21)),
-    (simp only: simps(22)),
-    (simp only: simps(23)),
-    (simp only: simps(24)),
-    (simp only: simps(25)),
-    (simp only: simps(26)),
-    (simp only: simps(27)),
-    (simp only: simps(28)),
-    (simp only: simps(29)),
-    (simp only: simps(30)),
-    (simp only: simps(31)),
-    (simp only: simps(32)),
-    (simp only: simps(33)),
-    (simp only: simps(34)),
-    (simp only: simps(35)),
-    (simp only: simps(36)),
-    (simp only: simps(37)),
-    (simp only: simps(38)),
-    (simp only: simps(39)),
-    (simp only: simps(40)),
-    (simp only: simps(41)),
-    (simp only: simps(42)),
-    (simp only: simps(43)),
-    (simp only: simps(44)),
-    (simp only: simps(45)),
-    (simp only: simps(46)))
+  \<open>\<And>p. check p \<equiv> prover [[(0,p)]]\<close>
+  \<open>\<And>h t. prover (h # t) \<equiv> prover (solves (h # t))\<close>
+  \<open>prover [] \<equiv> True\<close>
+  \<open>solves [] \<equiv> []\<close>
+  \<open>\<And>h t. solves (h # t) \<equiv> solve h @ solves t\<close>
+  \<open>solve [] \<equiv> [[]]\<close>
+  \<open>\<And>h t. solve (h # t) \<equiv> track t (fst h) (snd h)\<close>
+  \<open>\<And>s n b i v. track s n (Pre b i v) \<equiv> stop [s @ [(0,Pre b i v)]] (Pre (\<not> b) i v) (base s)\<close>
+  \<open>\<And>s n p q. track s n (Con p q) \<equiv> [s @ [(0,p)],s @ [(0,q)]]\<close>
+  \<open>\<And>s n p q. track s n (Dis p q) \<equiv> [s @ [(0,p),(0,q)]]\<close>
+  \<open>\<And>s n p. track s n (Uni p) \<equiv> [s @ [(0,subst 0 (fresh (frees (Uni p # base s))) p)]]\<close>
+  \<open>\<And>s n p. track s n (Exi p) \<equiv> [s @ [(0,subst 0 n p),(Suc n,Exi p)]]\<close>
+  \<open>\<And>c p. stop c p [] \<equiv> c\<close>
+  \<open>\<And>c p h t. stop c p (h # t) \<equiv> (if p = h then [] else stop c p t)\<close>
+  \<open>base [] \<equiv> []\<close>
+  \<open>\<And>h t. base (h # t) \<equiv> snd h # base t\<close>
+  \<open>\<And>x s b i v. subst x s (Pre b i v) \<equiv> Pre b i (mend x s v)\<close>
+  \<open>\<And>x s p q. subst x s (Con p q) \<equiv> Con (subst x s p) (subst x s q)\<close>
+  \<open>\<And>x s p q. subst x s (Dis p q) \<equiv> Dis (subst x s p) (subst x s q)\<close>
+  \<open>\<And>x s p. subst x s (Uni p) \<equiv> Uni (subst (Suc x) (Suc s) p)\<close>
+  \<open>\<And>x s p. subst x s (Exi p) \<equiv> Exi (subst (Suc x) (Suc s) p)\<close>
+  \<open>\<And>x s. mend x s [] \<equiv> []\<close>
+  \<open>\<And>x s h t. mend x s (h # t) \<equiv> more x s h (sub h x) # mend x s t\<close>
+  \<open>\<And>x s h. more x s h 0 \<equiv> over s h (sub x h)\<close>
+  \<open>\<And>x s h n. more x s h (Suc n) \<equiv> dec h\<close>
+  \<open>\<And>s h. over s h 0 \<equiv> s\<close>
+  \<open>\<And>s h n. over s h (Suc n) \<equiv> h\<close>
+  \<open>fresh [] \<equiv> 0\<close>
+  \<open>\<And>h t. fresh (h # t) \<equiv> Suc (add (sub (dec (fresh t)) h) h)\<close>
+  \<open>frees [] \<equiv> []\<close>
+  \<open>\<And>h t. frees (h # t) \<equiv> free h @ frees t\<close>
+  \<open>\<And>b i v. free (Pre b i v) \<equiv> v\<close>
+  \<open>\<And>p q. free (Con p q) \<equiv> free p @ free q\<close>
+  \<open>\<And>p q. free (Dis p q) \<equiv> free p @ free q\<close>
+  \<open>\<And>p. free (Uni p) \<equiv> dump (free p)\<close>
+  \<open>\<And>p. free (Exi p) \<equiv> dump (free p)\<close>
+  \<open>dump [] \<equiv> []\<close>
+  \<open>\<And>h t. dump (h # t) \<equiv> dash (dump t) h\<close>
+  \<open>\<And>l. dash l 0 \<equiv> l\<close>
+  \<open>\<And>l n. dash l (Suc n) \<equiv> n # l\<close>
+  by ((simp only: simps(1)),
+      (simp only: simps(2)),
+      (simp only: simps(3)),
+      (simp only: simps(4)),
+      (simp only: simps(5)),
+      (simp only: simps(6)),
+      (simp only: simps(7)),
+      (simp only: simps(8)),
+      (simp only: simps(9)),
+      (simp only: simps(10)),
+      (simp only: simps(11)),
+      (simp only: simps(12)),
+      (simp only: simps(13)),
+      (simp only: simps(14)),
+      (simp only: simps(15)),
+      (simp only: simps(16)),
+      (simp only: simps(17)),
+      (simp only: simps(18)),
+      (simp only: simps(19)),
+      (simp only: simps(20)),
+      (simp only: simps(21)),
+      (simp only: simps(22)),
+      (simp only: simps(23)),
+      (simp only: simps(24)),
+      (simp only: simps(25)),
+      (simp only: simps(26)),
+      (simp only: simps(27)),
+      (simp only: simps(28)),
+      (simp only: simps(29)),
+      (simp only: simps(30)),
+      (simp only: simps(31)),
+      (simp only: simps(32)),
+      (simp only: simps(33)),
+      (simp only: simps(34)),
+      (simp only: simps(35)),
+      (simp only: simps(36)),
+      (simp only: simps(37)),
+      (simp only: simps(38)),
+      (simp only: simps(39)),
+      (simp only: simps(40)))
 
 theorem data:
-  "\<And>b i v p q. Pre b i v = Con p q \<equiv> False"
-  "\<And>b i v p q. Con p q = Pre b i v \<equiv> False"
-  "\<And>b i v p q. Pre b i v = Dis p q \<equiv> False"
-  "\<And>b i v p q. Dis p q = Pre b i v \<equiv> False"
-  "\<And>b i v p. Pre b i v = Uni p \<equiv> False"
-  "\<And>b i v p. Uni p = Pre b i v \<equiv> False"
-  "\<And>b i v p. Pre b i v = Exi p \<equiv> False"
-  "\<And>b i v p. Exi p = Pre b i v \<equiv> False"
-  "\<And>p q p' q'. Con p q = Dis p' q' \<equiv> False"
-  "\<And>p q p' q'. Dis p' q' = Con p q \<equiv> False"
-  "\<And>p q p'. Con p q = Uni p' \<equiv> False"
-  "\<And>p q p'. Uni p' = Con p q \<equiv> False"
-  "\<And>p q p'. Con p q = Exi p' \<equiv> False"
-  "\<And>p q p'. Exi p' = Con p q \<equiv> False"
-  "\<And>p q p'. Dis p q = Uni p' \<equiv> False"
-  "\<And>p q p'. Uni p' = Dis p q \<equiv> False"
-  "\<And>p q p'. Dis p q = Exi p' \<equiv> False"
-  "\<And>p q p'. Exi p' = Dis p q \<equiv> False"
-  "\<And>p p'. Uni p = Exi p' \<equiv> False"
-  "\<And>p p'. Exi p' = Uni p \<equiv> False"
-  "\<And>b i v b' i' v'. Pre b i v = Pre b' i' v' \<equiv> b = b' \<and> i = i' \<and> v = v'"
-  "\<And>p q p' q'. Con p q = Con p' q' \<equiv> p = p' \<and> q = q'"
-  "\<And>p q p' q'. Dis p q = Dis p' q' \<equiv> p = p' \<and> q = q'"
-  "\<And>p p'. Uni p = Uni p' \<equiv> p = p'"
-  "\<And>p p'. Exi p = Exi p' \<equiv> p = p'"
-by ((simp only: simps(47)),
-    (simp only: simps(48)),
-    (simp only: simps(49)),
-    (simp only: simps(50)),
-    (simp only: simps(51)),
-    (simp only: simps(52)),
-    (simp only: simps(53)),
-    (simp only: simps(54)),
-    (simp only: simps(55)),
-    (simp only: simps(56)),
-    (simp only: simps(57)),
-    (simp only: simps(58)),
-    (simp only: simps(59)),
-    (simp only: simps(60)),
-    (simp only: simps(61)),
-    (simp only: simps(62)),
-    (simp only: simps(63)),
-    (simp only: simps(64)),
-    (simp only: simps(65)),
-    (simp only: simps(66)),
-    (simp only: simps(67)),
-    (simp only: simps(68)),
-    (simp only: simps(69)),
-    (simp only: simps(70)),
-    (simp only: simps(71)))
+  \<open>\<And>b i v p q. Pre b i v = Con p q \<equiv> False\<close>
+  \<open>\<And>b i v p q. Con p q = Pre b i v \<equiv> False\<close>
+  \<open>\<And>b i v p q. Pre b i v = Dis p q \<equiv> False\<close>
+  \<open>\<And>b i v p q. Dis p q = Pre b i v \<equiv> False\<close>
+  \<open>\<And>b i v p. Pre b i v = Uni p \<equiv> False\<close>
+  \<open>\<And>b i v p. Uni p = Pre b i v \<equiv> False\<close>
+  \<open>\<And>b i v p. Pre b i v = Exi p \<equiv> False\<close>
+  \<open>\<And>b i v p. Exi p = Pre b i v \<equiv> False\<close>
+  \<open>\<And>p q p' q'. Con p q = Dis p' q' \<equiv> False\<close>
+  \<open>\<And>p q p' q'. Dis p' q' = Con p q \<equiv> False\<close>
+  \<open>\<And>p q p'. Con p q = Uni p' \<equiv> False\<close>
+  \<open>\<And>p q p'. Uni p' = Con p q \<equiv> False\<close>
+  \<open>\<And>p q p'. Con p q = Exi p' \<equiv> False\<close>
+  \<open>\<And>p q p'. Exi p' = Con p q \<equiv> False\<close>
+  \<open>\<And>p q p'. Dis p q = Uni p' \<equiv> False\<close>
+  \<open>\<And>p q p'. Uni p' = Dis p q \<equiv> False\<close>
+  \<open>\<And>p q p'. Dis p q = Exi p' \<equiv> False\<close>
+  \<open>\<And>p q p'. Exi p' = Dis p q \<equiv> False\<close>
+  \<open>\<And>p p'. Uni p = Exi p' \<equiv> False\<close>
+  \<open>\<And>p p'. Exi p' = Uni p \<equiv> False\<close>
+  \<open>\<And>b i v b' i' v'. Pre b i v = Pre b' i' v' \<equiv> b = b' \<and> i = i' \<and> v = v'\<close>
+  \<open>\<And>p q p' q'. Con p q = Con p' q' \<equiv> p = p' \<and> q = q'\<close>
+  \<open>\<And>p q p' q'. Dis p q = Dis p' q' \<equiv> p = p' \<and> q = q'\<close>
+  \<open>\<And>p p'. Uni p = Uni p' \<equiv> p = p'\<close>
+  \<open>\<And>p p'. Exi p = Exi p' \<equiv> p = p'\<close>
+  by ((simp only: simps(41)),
+      (simp only: simps(42)),
+      (simp only: simps(43)),
+      (simp only: simps(44)),
+      (simp only: simps(45)),
+      (simp only: simps(46)),
+      (simp only: simps(47)),
+      (simp only: simps(48)),
+      (simp only: simps(49)),
+      (simp only: simps(50)),
+      (simp only: simps(51)),
+      (simp only: simps(52)),
+      (simp only: simps(53)),
+      (simp only: simps(54)),
+      (simp only: simps(55)),
+      (simp only: simps(56)),
+      (simp only: simps(57)),
+      (simp only: simps(58)),
+      (simp only: simps(59)),
+      (simp only: simps(60)),
+      (simp only: simps(61)),
+      (simp only: simps(62)),
+      (simp only: simps(63)),
+      (simp only: simps(64)),
+      (simp only: simps(65)))
 
 theorem library:
-  "\<And>l. [] @ l \<equiv> l"
-  "\<And>h t l. (h # t) @ l \<equiv> h # t @ l"
-  "\<And>x y. if True then x else y \<equiv> x"
-  "\<And>x y. if False then x else y \<equiv> y"
-  "\<not> True \<equiv> False"
-  "\<not> False \<equiv> True"
-  "\<And>x y. fst (x,y) \<equiv> x"
-  "\<And>x y. snd (x,y) \<equiv> y"
-  "\<And>n. 0 = Suc n \<equiv> False"
-  "\<And>n. Suc n = 0 \<equiv> False"
-  "\<And>h t. [] = h # t \<equiv> False"
-  "\<And>h t. h # t = [] \<equiv> False"
-  "True = False \<equiv> False"
-  "False = True \<equiv> False"
-  "0 = 0 \<equiv> True"
-  "[] = [] \<equiv> True"
-  "True = True \<equiv> True"
-  "False = False \<equiv> True"
-  "\<And>x y x' y'. (x,y) = (x',y') \<equiv> x = x' \<and> y = y'"
-  "\<And>n n'. Suc n = Suc n' \<equiv> n = n'"
-  "\<And>h t h' t'. h # t = h' # t' \<equiv> h = h' \<and> t = t'"
-  "\<And>b. True \<and> b \<equiv> b"
-  "\<And>b. False \<and> b \<equiv> False"
-by ((simp only: simps(72)),
-    (simp only: simps(73)),
-    (simp only: simps(74)),
-    (simp only: simps(75)),
-    (simp only: simps(76)),
-    (simp only: simps(77)),
-    (simp only: simps(78)),
-    (simp only: simps(79)),
-    (simp only: simps(80)),
-    (simp only: simps(81)),
-    (simp only: simps(82)),
-    (simp only: simps(83)),
-    (simp only: simps(84)),
-    (simp only: simps(85)),
-    (simp only: simps(86)),
-    (simp only: simps(87)),
-    (simp only: simps(88)),
-    (simp only: simps(89)),
-    (simp only: simps(90)),
-    (simp only: simps(91)),
-    (simp only: simps(92)),
-    (simp only: simps(93)),
-    (simp only: simps(94)))
+  \<open>\<And>x. add x 0 \<equiv> x\<close>
+  \<open>\<And>x n. add x (Suc n) \<equiv> Suc (add x n)\<close>
+  \<open>\<And>x. sub x 0 \<equiv> x\<close>
+  \<open>\<And>x n. sub x (Suc n) \<equiv> dec (sub x n)\<close>
+  \<open>dec 0 \<equiv> 0\<close>
+  \<open>\<And>n. dec (Suc n) \<equiv> n\<close>
+  \<open>\<And>l. [] @ l \<equiv> l\<close>
+  \<open>\<And>h t l. (h # t) @ l \<equiv> h # t @ l\<close>
+  \<open>\<And>x y. if True then x else y \<equiv> x\<close>
+  \<open>\<And>x y. if False then x else y \<equiv> y\<close>
+  \<open>\<not> True \<equiv> False\<close>
+  \<open>\<not> False \<equiv> True\<close>
+  \<open>\<And>x y. fst (x,y) \<equiv> x\<close>
+  \<open>\<And>x y. snd (x,y) \<equiv> y\<close>
+  \<open>0 = 0 \<equiv> True\<close>
+  \<open>[] = [] \<equiv> True\<close>
+  \<open>True = True \<equiv> True\<close>
+  \<open>False = False \<equiv> True\<close>
+  \<open>\<And>b. True \<and> b \<equiv> b\<close>
+  \<open>\<And>b. False \<and> b \<equiv> False\<close>
+  \<open>\<And>n. 0 = Suc n \<equiv> False\<close>
+  \<open>\<And>n. Suc n = 0 \<equiv> False\<close>
+  \<open>\<And>h t. [] = h # t \<equiv> False\<close>
+  \<open>\<And>h t. h # t = [] \<equiv> False\<close>
+  \<open>True = False \<equiv> False\<close>
+  \<open>False = True \<equiv> False\<close>
+  \<open>\<And>x y x' y'. (x,y) = (x',y') \<equiv> x = x' \<and> y = y'\<close>
+  \<open>\<And>n n'. Suc n = Suc n' \<equiv> n = n'\<close>
+  \<open>\<And>h t h' t'. h # t = h' # t' \<equiv> h = h' \<and> t = t'\<close>
+  by ((simp only: simps(66)),
+      (simp only: simps(67)),
+      (simp only: simps(68)),
+      (simp only: simps(69)),
+      (simp only: simps(70)),
+      (simp only: simps(71)),
+      (simp only: simps(72)),
+      (simp only: simps(73)),
+      (simp only: simps(74)),
+      (simp only: simps(75)),
+      (simp only: simps(76)),
+      (simp only: simps(77)),
+      (simp only: simps(78)),
+      (simp only: simps(79)),
+      (simp only: simps(80)),
+      (simp only: simps(81)),
+      (simp only: simps(82)),
+      (simp only: simps(83)),
+      (simp only: simps(84)),
+      (simp only: simps(85)),
+      (simp only: simps(86)),
+      (simp only: simps(87)),
+      (simp only: simps(88)),
+      (simp only: simps(89)),
+      (simp only: simps(90)),
+      (simp only: simps(91)),
+      (simp only: simps(92)),
+      (simp only: simps(93)),
+      (simp only: simps(94)))
 
-proposition "check test"
-unfolding test_def
-unfolding program(1)
-unfolding program(2)
-unfolding program(3-) data library
-unfolding program(2)
-unfolding program(3-) data library
-unfolding program(2)
-unfolding program(3-) data library
-unfolding program(2)
-unfolding program(3-) data library
-unfolding program(2)
-unfolding program(3-) data library
-unfolding program(2)
-unfolding program(3-) data library
-unfolding program(2)
-unfolding program(3-) data library
-by (rule TrueI)
+proposition \<open>check test\<close>
+  unfolding test_def
+  unfolding program(1)
+  unfolding program(2)
+  unfolding program(3-) data library
+  unfolding program(2)
+  unfolding program(3-) data library
+  unfolding program(2)
+  unfolding program(3-) data library
+  unfolding program(2)
+  unfolding program(3-) data library
+  unfolding program(2)
+  unfolding program(3-) data library
+  unfolding program(2)
+  unfolding program(3-) data library
+  unfolding program(2)
+  unfolding program(3-) data library
+  by (rule TrueI)
 
-proposition "check test"
-unfolding check_def
-unfolding main_def
-unfolding test_def
-by (simp add: iterator)
+proposition \<open>check test\<close>
+  unfolding check_def
+  unfolding main_def
+  unfolding test_def
+  by (simp add: iterator)
 
-proposition "check test"
-by code_simp
+proposition \<open>check test\<close>
+  by code_simp
 
-proposition "map length (map (repeat (solves) [[(0,test)]]) [1,2,3,4,5,6,7]) = [1,1,1,2,2,2,0]"
-by code_simp
+proposition \<open>map length (map (repeat (solves) [[(0,test)]]) [1,2,3,4,5,6,7]) = [1,1,1,2,2,2,0]\<close>
+  by code_simp
 
-proposition "repeat (solves) [[(0,test)]] (Suc (Suc (Suc (Suc (Suc (Suc (Suc 0))))))) = []"
-unfolding repeat.simps
-unfolding test_def
-unfolding program data library
-by (rule TrueI)
+proposition \<open>repeat (solves) [[(0,test)]] (Suc (Suc (Suc (Suc (Suc (Suc (Suc 0))))))) = []\<close>
+  unfolding repeat.simps
+  unfolding test_def
+  unfolding program data library
+  by (rule TrueI)
 
-proposition "\<forall>m e. is_model_environment m e \<longrightarrow> fst m \<noteq> {}"
-unfolding is_model_environment_def
-by fast
+proposition \<open>\<forall>m e. is_model_environment m e \<longrightarrow> fst m \<noteq> {}\<close>
+  unfolding is_model_environment_def
+  by fast
 
-inductive_set calculation :: "sequent \<Rightarrow> (nat \<times> sequent) set" for s where
-  "(0,s) \<in> calculation s" |
-  "(n,k) \<in> calculation s \<Longrightarrow> l \<in> set (solve k) \<Longrightarrow> (Suc n,l) \<in> calculation s"
+inductive_set calculation :: \<open>sequent \<Rightarrow> (nat \<times> sequent) set\<close> for s where
+  \<open>(0,s) \<in> calculation s\<close> |
+  \<open>(n,k) \<in> calculation s \<Longrightarrow> l \<in> set (solve k) \<Longrightarrow> (Suc n,l) \<in> calculation s\<close>
 
-primrec semantics_alternative :: "model \<Rightarrow> environment \<Rightarrow> nnf list \<Rightarrow> bool" where
-  "semantics_alternative _ _ [] = False" |
-  "semantics_alternative m e (h # t) = (semantics m e h \<or> semantics_alternative m e t)"
+primrec semantics_alternative :: \<open>model \<Rightarrow> environment \<Rightarrow> nnf list \<Rightarrow> bool\<close> where
+  \<open>semantics_alternative _ _ [] = False\<close> |
+  \<open>semantics_alternative m e (h # t) = (semantics m e h \<or> semantics_alternative m e t)\<close>
 
-definition valid :: "nnf list \<Rightarrow> bool" where
-  "valid l \<equiv> \<forall>m e. is_model_environment m e \<longrightarrow> semantics_alternative m e l"
+definition valid :: \<open>nnf list \<Rightarrow> bool\<close> where
+  \<open>valid l \<equiv> \<forall>m e. is_model_environment m e \<longrightarrow> semantics_alternative m e l\<close>
 
-abbreviation (input) "VALID \<equiv> valid = finite \<circ> calculation \<circ> map (Pair 0)"
+abbreviation (input) \<open>VALID \<equiv> valid = finite \<circ> calculation \<circ> map (Pair 0)\<close>
 
-section "Soundness and Completeness"
+section \<open>Soundness and Completeness\<close>
 
-subsection "Basics"
+subsection \<open>Basics\<close>
 
-primrec increase :: "(nat \<Rightarrow> nat) \<Rightarrow> nat \<Rightarrow> nat" where
-  "increase _ 0 = 0" |
-  "increase f (Suc n) = Suc (f n)"
+primrec increase :: \<open>(nat \<Rightarrow> nat) \<Rightarrow> nat \<Rightarrow> nat\<close> where
+  \<open>increase _ 0 = 0\<close> |
+  \<open>increase f (Suc n) = Suc (f n)\<close>
 
-primrec sv :: "(nat \<Rightarrow> nat) \<Rightarrow> nnf \<Rightarrow> nnf" where
-  "sv f (Pre b i v) = Pre b i (map f v)" |
-  "sv f (Con p q) = Con (sv f p) (sv f q)" |
-  "sv f (Dis p q) = Dis (sv f p) (sv f q)" |
-  "sv f (Uni p) = Uni (sv (increase f) p)" |
-  "sv f (Exi p) = Exi (sv (increase f) p)"
+primrec sv :: \<open>(nat \<Rightarrow> nat) \<Rightarrow> nnf \<Rightarrow> nnf\<close> where
+  \<open>sv f (Pre b i v) = Pre b i (map f v)\<close> |
+  \<open>sv f (Con p q) = Con (sv f p) (sv f q)\<close> |
+  \<open>sv f (Dis p q) = Dis (sv f p) (sv f q)\<close> |
+  \<open>sv f (Uni p) = Uni (sv (increase f) p)\<close> |
+  \<open>sv f (Exi p) = Exi (sv (increase f) p)\<close>
 
-primrec bind :: "nat \<Rightarrow> nat \<Rightarrow> nat" where
-  "bind x 0 = x" |
-  "bind _ (Suc n) = n"
+primrec bind :: \<open>nat \<Rightarrow> nat \<Rightarrow> nat\<close> where
+  \<open>bind x 0 = x\<close> |
+  \<open>bind _ (Suc n) = n\<close>
 
-definition inst :: "nnf \<Rightarrow> nat \<Rightarrow> nnf" where
-  "inst p x \<equiv> sv (bind x) p"
+definition inst :: \<open>nnf \<Rightarrow> nat \<Rightarrow> nnf\<close> where
+  \<open>inst p x \<equiv> sv (bind x) p\<close>
 
-lemma j1: "(if h < x then h else if h = x then s else h - 1) =
- (if h - x = 0 then (if x - h = 0 then s else h) else dec h)" for h :: nat
+lemma j1: \<open>(if h < x then h else if h = x then s else h - 1) =
+ (if h - x = 0 then (if x - h = 0 then s else h) else dec h)\<close> for h :: nat
 proof -
   obtain bb :: bool where
-    f1: "bb = (h - x = 0 \<longrightarrow> (x - h = 0 \<longrightarrow> (h < x \<longrightarrow> h = s) \<and> (\<not> h < x \<longrightarrow> h \<noteq> x \<longrightarrow> h - 1 = s))
-        \<and> (x - h \<noteq> 0 \<longrightarrow> \<not> h < x \<longrightarrow> (h = x \<longrightarrow> s = h) \<and> (h \<noteq> x \<longrightarrow> h - 1 = h)))"
+    f1: \<open>bb = (h - x = 0 \<longrightarrow> (x - h = 0 \<longrightarrow> (h < x \<longrightarrow> h = s) \<and> (\<not> h < x \<longrightarrow> h \<noteq> x \<longrightarrow> h - 1 = s))
+        \<and> (x - h \<noteq> 0 \<longrightarrow> \<not> h < x \<longrightarrow> (h = x \<longrightarrow> s = h) \<and> (h \<noteq> x \<longrightarrow> h - 1 = h)))\<close>
     by metis
-  then have "bb \<and> (h - x = 0 \<or> (\<not> h < x \<or> h = dec h) \<and> (h < x \<or> (h \<noteq> x \<or> s = dec h)
-            \<and> (h = x \<or> h - 1 = dec h)))"
+  then have \<open>bb \<and> (h - x = 0 \<or> (\<not> h < x \<or> h = dec h) \<and> (h < x \<or> (h \<noteq> x \<or> s = dec h)
+            \<and> (h = x \<or> h - 1 = dec h)))\<close>
     by (metis dec.simps(2) diff_Suc_1 diffs0_imp_equal less_SucI not_less_eq old.nat.exhaust
         zero_less_Suc zero_less_diff)
   then show ?thesis
     using f1 by presburger
 qed
 
-lemma j2: "(sub h x) = (h - x)" for h :: nat
+lemma j2: \<open>(sub h x) = (h - x)\<close> for h :: nat
   by (induct x) (simp_all,simp add: nat_diff_split)
 
-lemma j3: "(if h < x then h else if h = x then s else h - 1) = (if sub h x = 0 then
-          (if sub x h = 0 then s else h) else dec h)" for h :: nat
+lemma j3: \<open>(if h < x then h else if h = x then s else h - 1) = (if sub h x = 0 then
+          (if sub x h = 0 then s else h) else dec h)\<close> for h :: nat
   by (simp add: j1 j2)
 
-lemma j4: "more x s h (sub h x) = (if sub h x = 0 then (if sub x h = 0 then s else h) else dec h)"
+lemma j4: \<open>more x s h (sub h x) = (if sub h x = 0 then (if sub x h = 0 then s else h) else dec h)\<close>
   for h :: nat
   by (metis over.simps(1) over.simps(2) more.simps(1) more.simps(2) old.nat.exhaust)
 
-lemma j5: "mend x s v = map (\<lambda>n. (if n < x then n else if n = x then s else n - 1)) v"
+lemma j5: \<open>mend x s v = map (\<lambda>n. (if n < x then n else if n = x then s else n - 1)) v\<close>
   by (induct v) (simp_all add: j4,simp add: j2 nat_diff_split)
 
-definition instt :: "nnf \<Rightarrow> nat \<Rightarrow> nnf" where
-  "instt p x \<equiv> subst 0 x p"
+definition instt :: \<open>nnf \<Rightarrow> nat \<Rightarrow> nnf\<close> where
+  \<open>instt p x \<equiv> subst 0 x p\<close>
 
-primrec increases :: "nat \<Rightarrow> (nat \<Rightarrow> nat) \<Rightarrow> (nat \<Rightarrow> nat)" where
-  "increases 0 x = x" |
-  "increases (Suc n) x = increase (increases n x)"
+primrec increases :: \<open>nat \<Rightarrow> (nat \<Rightarrow> nat) \<Rightarrow> (nat \<Rightarrow> nat)\<close> where
+  \<open>increases 0 x = x\<close> |
+  \<open>increases (Suc n) x = increase (increases n x)\<close>
 
 lemma increases_bind:
-  "(\<lambda>n. (if n < m then n else if n = m then x + m else n - 1)) n = increases m (bind x) n"
+  \<open>(\<lambda>n. (if n < m then n else if n = m then x + m else n - 1)) n = increases m (bind x) n\<close>
 proof (induct m arbitrary: n)
   case 0
   then show ?case
     by (induct n) simp_all
 next
   case (Suc k)
-  then have "increases (Suc k) (bind x) n =
-      increase (\<lambda>n. if n < k then n else if n = k then x + k else n - 1) n"
+  then have \<open>increases (Suc k) (bind x) n =
+      increase (\<lambda>n. if n < k then n else if n = k then x + k else n - 1) n\<close>
     by simp
   then show ?case
     by (induct n) simp_all
 qed
 
-lemma subb_sv: "subst m (x + m) p = sv (increases m (bind x)) p"
+lemma subb_sv: \<open>subst m (x + m) p = sv (increases m (bind x)) p\<close>
 proof (induct p arbitrary: m)
   case (Pre b i v)
   then show ?case
@@ -535,155 +537,155 @@ next
     by simp
 next
   case (Uni p)
-  have "subst m (x + m) (Uni p) = Uni (subst (Suc m) (x + Suc m) p)"
+  have \<open>subst m (x + m) (Uni p) = Uni (subst (Suc m) (x + Suc m) p)\<close>
     by simp
-  also have "\<dots> = Uni (sv (increases (Suc m) (bind x)) p)"
+  also have \<open>\<dots> = Uni (sv (increases (Suc m) (bind x)) p)\<close>
     using Uni by blast
-  also have "\<dots> = sv (increases m (bind x)) (Uni p)"
+  also have \<open>\<dots> = sv (increases m (bind x)) (Uni p)\<close>
     by simp
   finally show ?case .
 next
   case (Exi p)
-  have "subst m (x + m) (Exi p) = Exi (subst (Suc m) (x + Suc m) p)"
+  have \<open>subst m (x + m) (Exi p) = Exi (subst (Suc m) (x + Suc m) p)\<close>
     by simp
-  also have "\<dots> = Exi (sv (increases (Suc m) (bind x)) p)"
+  also have \<open>\<dots> = Exi (sv (increases (Suc m) (bind x)) p)\<close>
     using Exi by blast
- also have "\<dots> = sv (increases m (bind x)) (Exi p)"
-   by simp
+  also have \<open>\<dots> = sv (increases m (bind x)) (Exi p)\<close>
+    by simp
   finally show ?case .
 qed
 
-lemma instt: "instt p x = inst p x"
+lemma instt: \<open>instt p x = inst p x\<close>
   unfolding inst_def instt_def
   using subb_sv by (metis add_cancel_left_right increases.simps(1))
 
-lemma base: "base s = map snd s"
+lemma base: \<open>base s = map snd s\<close>
   by (induct s) simp_all
 
-definition maps :: "('a \<Rightarrow> 'b list) \<Rightarrow> 'a list \<Rightarrow> 'b list" where
-  "maps f l \<equiv> concat (map f l)"
+definition maps :: \<open>('a \<Rightarrow> 'b list) \<Rightarrow> 'a list \<Rightarrow> 'b list\<close> where
+  \<open>maps f l \<equiv> concat (map f l)\<close>
 
-lemma frees: "frees l = maps free l"
+lemma frees: \<open>frees l = maps free l\<close>
   unfolding maps_def by (induct l) simp_all
 
-lemma solves: "solves l = maps solve l"
+lemma solves: \<open>solves l = maps solve l\<close>
   unfolding maps_def by (induct l) simp_all
 
-lemma ms: "maps solve = solves"
-using ext solves by fastforce
+lemma ms: \<open>maps solve = solves\<close>
+  using ext solves by fastforce
 
-primrec maxl :: "nat list \<Rightarrow> nat" where
-  "maxl [] = 0" |
-  "maxl (h # t) = add (sub (maxl t) h) h"
+primrec maxl :: \<open>nat list \<Rightarrow> nat\<close> where
+  \<open>maxl [] = 0\<close> |
+  \<open>maxl (h # t) = add (sub (maxl t) h) h\<close>
 
-definition fresh' :: "nat list \<Rightarrow> nat" where
-  "fresh' l \<equiv> if null l then 0 else Suc (maxl l)"
+definition fresh' :: \<open>nat list \<Rightarrow> nat\<close> where
+  \<open>fresh' l \<equiv> if null l then 0 else Suc (maxl l)\<close>
 
-lemma fresh': "fresh l = fresh' l"
-unfolding fresh'_def by (induct l) (auto, metis null.simps(2) list.exhaust maxl.simps)
+lemma fresh': \<open>fresh l = fresh' l\<close>
+  unfolding fresh'_def by (induct l) (auto, metis null.simps(2) list.exhaust maxl.simps)
 
-primrec repeat' :: "('a \<Rightarrow> 'a) \<Rightarrow> 'a \<Rightarrow> nat \<Rightarrow> 'a" where
-  "repeat' _ c 0 = c" |
-  "repeat' f c (Suc n) = f (repeat' f c n)"
+primrec repeat' :: \<open>('a \<Rightarrow> 'a) \<Rightarrow> 'a \<Rightarrow> nat \<Rightarrow> 'a\<close> where
+  \<open>repeat' _ c 0 = c\<close> |
+  \<open>repeat' f c (Suc n) = f (repeat' f c n)\<close>
 
-lemma r: "f (repeat f c n) = repeat f (f c) n"
-by (induct n arbitrary: c) simp_all
+lemma r: \<open>f (repeat f c n) = repeat f (f c) n\<close>
+  by (induct n arbitrary: c) simp_all
 
-lemma rr: "repeat' f c n = repeat f c n"
-by (induct n) (simp_all add: r)
+lemma rr: \<open>repeat' f c n = repeat f c n\<close>
+  by (induct n) (simp_all add: r)
 
-primrec sub' :: "nat \<Rightarrow> nat \<Rightarrow> nat" where
-  "sub' x 0 = x" |
-  "sub' x (Suc n) = sub' (dec x) n"
+primrec sub' :: \<open>nat \<Rightarrow> nat \<Rightarrow> nat\<close> where
+  \<open>sub' x 0 = x\<close> |
+  \<open>sub' x (Suc n) = sub' (dec x) n\<close>
 
-lemma d0: "dec x = x-(1::nat)"
-by (simp add: nat_diff_split)
+lemma d0: \<open>dec x = x-(1::nat)\<close>
+  by (simp add: nat_diff_split)
 
-lemma d1: "sub' x y = x-(y::nat)"
-using d0 diff_Suc_eq_diff_pred sub'.simps by (induct y arbitrary: x) presburger+
+lemma d1: \<open>sub' x y = x-(y::nat)\<close>
+  using d0 diff_Suc_eq_diff_pred sub'.simps by (induct y arbitrary: x) presburger+
 
-lemma dx: "sub x y = sub' x y"
-by (simp add: d1 j2)
+lemma dx: \<open>sub x y = sub' x y\<close>
+  by (simp add: d1 j2)
 
-lemma mmm: "(add (sub n n') n') = (max n n')"
+lemma mmm: \<open>(add (sub n n') n') = (max n n')\<close>
 proof (induct n' arbitrary: n)
   case 0 then show ?case by simp
 next
   case Suc then show ?case
   proof -
     fix n'a :: nat and na :: nat
-    assume a1: "\<And>n. add (sub n n'a) n'a = max n n'a"
-    have f2: "\<And>n na. n = 0 \<or> Suc (max na (n - 1)) = max (Suc na) n"
+    assume a1: \<open>\<And>n. add (sub n n'a) n'a = max n n'a\<close>
+    have f2: \<open>\<And>n na. n = 0 \<or> Suc (max na (n - 1)) = max (Suc na) n\<close>
       by (metis (lifting) Nitpick.case_nat_unfold max_Suc1)
-    { assume "na \<noteq> 0"
-      then have "Suc (max n'a (dec na)) = max na (Suc n'a)"
+    { assume \<open>na \<noteq> 0\<close>
+      then have \<open>Suc (max n'a (dec na)) = max na (Suc n'a)\<close>
         using f2 by (metis (lifting) dec.simps(2) Suc_pred' max.commute not_gr0) }
-    then have "Suc (max n'a (dec na)) = max na (Suc n'a)"
+    then have \<open>Suc (max n'a (dec na)) = max na (Suc n'a)\<close>
       by (metis max.commute max_0L dec.simps(1))
-    then show "add (sub na (Suc n'a)) (Suc n'a) = max na (Suc n'a)"
+    then show \<open>add (sub na (Suc n'a)) (Suc n'a) = max na (Suc n'a)\<close>
       using a1 dx by simp
   qed
 qed
 
-lemma maps: "maps f = (concat \<circ> map f)"
-using maps_def comp_apply
-by fastforce
+lemma maps: \<open>maps f = (concat \<circ> map f)\<close>
+  using maps_def comp_apply
+  by fastforce
 
-definition make_sequent :: "nnf list \<Rightarrow> sequent" where
-  "make_sequent l = map (\<lambda>p. (0,p)) l"
+definition make_sequent :: \<open>nnf list \<Rightarrow> sequent\<close> where
+  \<open>make_sequent l = map (\<lambda>p. (0,p)) l\<close>
 
-definition list_sequent :: "sequent \<Rightarrow> nnf list" where
-  "list_sequent s = map snd s"
+definition list_sequent :: \<open>sequent \<Rightarrow> nnf list\<close> where
+  \<open>list_sequent s = map snd s\<close>
 
-definition fv_list :: "nnf list \<Rightarrow> nat list" where
-  "fv_list \<equiv> maps free"
+definition fv_list :: \<open>nnf list \<Rightarrow> nat list\<close> where
+  \<open>fv_list \<equiv> maps free\<close>
 
-primrec is_axiom :: "nnf list \<Rightarrow> bool" where
-  "is_axiom [] = False" |
-  "is_axiom (p # t) = ((\<exists>b i v. p = Pre b i v \<and> Pre (\<not> b) i v \<in> set t))"
+primrec is_axiom :: \<open>nnf list \<Rightarrow> bool\<close> where
+  \<open>is_axiom [] = False\<close> |
+  \<open>is_axiom (p # t) = ((\<exists>b i v. p = Pre b i v \<and> Pre (\<not> b) i v \<in> set t))\<close>
 
-primrec member :: "'a \<Rightarrow> 'a list \<Rightarrow> bool" where
-  "member _ [] = False" |
-  "member a (h # t) = (if a = h then True else member a t)"
+primrec member :: \<open>'a \<Rightarrow> 'a list \<Rightarrow> bool\<close> where
+  \<open>member _ [] = False\<close> |
+  \<open>member a (h # t) = (if a = h then True else member a t)\<close>
 
-lemma member_set: "member a l = (a \<in> set l)"
-by (induct l) auto
+lemma member_set: \<open>member a l = (a \<in> set l)\<close>
+  by (induct l) auto
 
-lemma stop: "stop [t @ [(0,r)]] (Pre (\<not> b) i v) l =
-  (if member (Pre (\<not> b) i v) l then [] else [t @ [(0,r)]])"
-by (induct l) simp_all
+lemma stop: \<open>stop [t @ [(0,r)]] (Pre (\<not> b) i v) l =
+  (if member (Pre (\<not> b) i v) l then [] else [t @ [(0,r)]])\<close>
+  by (induct l) simp_all
 
-lemma pre: "(n,(m,Pre b i v) # xs) \<in> calculation(nfs) \<Longrightarrow>
+lemma pre: \<open>(n,(m,Pre b i v) # xs) \<in> calculation(nfs) \<Longrightarrow>
     \<not> is_axiom (list_sequent ((m,Pre b i v) # xs)) \<Longrightarrow>
-    (Suc n,xs@[(0,Pre b i v)]) \<in> calculation(nfs)"
-  and con1: "(n,(m,Con p q) # xs) \<in> calculation(nfs) \<Longrightarrow>
+    (Suc n,xs@[(0,Pre b i v)]) \<in> calculation(nfs)\<close>
+  and con1: \<open>(n,(m,Con p q) # xs) \<in> calculation(nfs) \<Longrightarrow>
     \<not> is_axiom (list_sequent ((m,Con p q) # xs)) \<Longrightarrow>
-    (Suc n,xs@[(0,p)]) \<in> calculation(nfs)"
-  and con2: "(n,(m,Con p q) # xs) \<in> calculation(nfs) \<Longrightarrow>
+    (Suc n,xs@[(0,p)]) \<in> calculation(nfs)\<close>
+  and con2: \<open>(n,(m,Con p q) # xs) \<in> calculation(nfs) \<Longrightarrow>
     \<not> is_axiom (list_sequent ((m,Con p q) # xs)) \<Longrightarrow>
-    (Suc n,xs@[(0,q)]) \<in> calculation(nfs)"
-  and dis: "(n,(m,Dis p q) # xs) \<in> calculation(nfs) \<Longrightarrow>
+    (Suc n,xs@[(0,q)]) \<in> calculation(nfs)\<close>
+  and dis: \<open>(n,(m,Dis p q) # xs) \<in> calculation(nfs) \<Longrightarrow>
     \<not> is_axiom (list_sequent ((m,Dis p q) # xs)) \<Longrightarrow>
-    (Suc n,xs@[(0,p),(0,q)]) \<in> calculation(nfs)"
-  and uni: "(n,(m,Uni p) # xs) \<in> calculation(nfs) \<Longrightarrow>
+    (Suc n,xs@[(0,p),(0,q)]) \<in> calculation(nfs)\<close>
+  and uni: \<open>(n,(m,Uni p) # xs) \<in> calculation(nfs) \<Longrightarrow>
     \<not> is_axiom (list_sequent ((m,Uni p) # xs)) \<Longrightarrow>
     (Suc n,xs@[(0,sv (bind (fresh ((concat \<circ> map free) (list_sequent ((m,Uni p) # xs))))) p)])
-      \<in> calculation(nfs)"
-  and exi: "(n,(m,Exi p) # xs) \<in> calculation(nfs) \<Longrightarrow>
+      \<in> calculation(nfs)\<close>
+  and exi: \<open>(n,(m,Exi p) # xs) \<in> calculation(nfs) \<Longrightarrow>
     \<not> is_axiom (list_sequent ((m,Exi p) # xs)) \<Longrightarrow>
-    (Suc n,xs@[(0,sv (bind m) p),(Suc m,Exi p)]) \<in> calculation(nfs)"
-using instt_def
-by (auto simp: instt list_sequent_def maps inst_def stop member_set calculation.intros base frees)
+    (Suc n,xs@[(0,sv (bind m) p),(Suc m,Exi p)]) \<in> calculation(nfs)\<close>
+  using instt_def
+  by (auto simp: instt list_sequent_def maps inst_def stop member_set calculation.intros base frees)
 
 lemmas not_is_axiom_subs = pre con1 con2 dis uni exi
 
-lemma calculation_init: "(0,k) \<in> calculation s = (k = s)"
-using calculation.simps
-by blast
+lemma calculation_init: \<open>(0,k) \<in> calculation s = (k = s)\<close>
+  using calculation.simps
+  by blast
 
 lemma calculation_upwards:
-  assumes "(n,k) \<in> calculation s" and "\<not> is_axiom (list_sequent (k))"
-  shows "(\<exists>l. (Suc n,l) \<in> calculation s \<and> l \<in> set (solve k))"
+  assumes \<open>(n,k) \<in> calculation s\<close> and \<open>\<not> is_axiom (list_sequent (k))\<close>
+  shows \<open>(\<exists>l. (Suc n,l) \<in> calculation s \<and> l \<in> set (solve k))\<close>
 proof (cases k)
   case Nil then show ?thesis using assms(1) calculation.intros(2) by auto
 next
@@ -691,21 +693,21 @@ next
   proof (cases a)
     case (Pair _ p) then show ?thesis
       using Cons assms calculation.intros(2)
-        by (cases p) (fastforce simp: list_sequent_def stop member_set base)+
+      by (cases p) (fastforce simp: list_sequent_def stop member_set base)+
   qed
 qed
 
-lemma calculation_downwards: "(Suc n,k) \<in> calculation s \<Longrightarrow>
-  \<exists>t. (n,t) \<in> calculation s \<and> k \<in> set (solve t) \<and> \<not> is_axiom (list_sequent t)"
+lemma calculation_downwards: \<open>(Suc n,k) \<in> calculation s \<Longrightarrow>
+  \<exists>t. (n,t) \<in> calculation s \<and> k \<in> set (solve t) \<and> \<not> is_axiom (list_sequent t)\<close>
 proof (erule calculation.cases)
-  assume "Suc n = 0"
+  assume \<open>Suc n = 0\<close>
   then show ?thesis using list_sequent_def by simp
 next
   fix m l k'
-  assume 1: "Suc n = Suc m"
-  and 2: "k = k'"
-  and 3: "(m,l) \<in> calculation s"
-  and 4: "k' \<in> set (solve l)"
+  assume 1: \<open>Suc n = Suc m\<close>
+    and 2: \<open>k = k'\<close>
+    and 3: \<open>(m,l) \<in> calculation s\<close>
+    and 4: \<open>k' \<in> set (solve l)\<close>
   then show ?thesis
   proof (cases l)
     case Nil then show ?thesis using 1 2 3 4 list_sequent_def by fastforce
@@ -719,113 +721,113 @@ next
 qed
 
 lemma calculation_calculation_child:
-  "\<forall>s t. (Suc n,s) \<in> calculation t =
-    (\<exists>k. k \<in> set (solve t) \<and> \<not> is_axiom (list_sequent t) \<and> (n,s) \<in> calculation k)"
-by (induct n) (metis calculation.intros(2) calculation_downwards calculation_init,
-    meson calculation.intros(2) calculation_downwards)
+  \<open>\<forall>s t. (Suc n,s) \<in> calculation t =
+    (\<exists>k. k \<in> set (solve t) \<and> \<not> is_axiom (list_sequent t) \<and> (n,s) \<in> calculation k)\<close>
+  by (induct n) (metis calculation.intros(2) calculation_downwards calculation_init,
+      meson calculation.intros(2) calculation_downwards)
 
 lemma calculation_progress:
-  assumes "(n,a # l) \<in> calculation s" and "\<not> is_axiom (list_sequent (a # l))"
-  shows "(\<exists>k. (Suc n,l@k) \<in> calculation s)"
+  assumes \<open>(n,a # l) \<in> calculation s\<close> and \<open>\<not> is_axiom (list_sequent (a # l))\<close>
+  shows \<open>(\<exists>k. (Suc n,l@k) \<in> calculation s)\<close>
 proof (cases a)
   case (Pair _ p) then show ?thesis using assms by (cases p) (auto dest: not_is_axiom_subs)
 qed
 
-definition inc :: "nat \<times> sequent \<Rightarrow> nat \<times> sequent" where
-  "inc \<equiv> \<lambda>(n,fs). (Suc n,fs)"
+definition inc :: \<open>nat \<times> sequent \<Rightarrow> nat \<times> sequent\<close> where
+  \<open>inc \<equiv> \<lambda>(n,fs). (Suc n,fs)\<close>
 
-lemma inj_inc: "inj inc"
-by (simp add: inc_def inj_on_def)
+lemma inj_inc: \<open>inj inc\<close>
+  by (simp add: inc_def inj_on_def)
 
-lemma calculation: "calculation s =
-  insert (0,s) (inc ` (\<Union> (calculation ` {k. \<not> is_axiom (list_sequent s) \<and> k \<in> set (solve s)})))"
+lemma calculation: \<open>calculation s =
+  insert (0,s) (inc ` (\<Union> (calculation ` {k. \<not> is_axiom (list_sequent s) \<and> k \<in> set (solve s)})))\<close>
 proof (rule set_eqI,simp add: split_paired_all)
   fix n k
-  show "((n,k) \<in> calculation s) =
+  show \<open>((n,k) \<in> calculation s) =
     (n = 0 \<and> k = s \<or> (n,k) \<in> inc ` (\<Union>x\<in>{k. \<not> is_axiom (list_sequent s) \<and> k \<in> set (solve s)}.
-      calculation x))"
-  by (cases n) (auto simp: calculation_init calculation_calculation_child inc_def)
+      calculation x))\<close>
+    by (cases n) (auto simp: calculation_init calculation_calculation_child inc_def)
 qed
 
 lemma calculation_is_axiom:
-  assumes "is_axiom (list_sequent s)"
-  shows "calculation s = {(0,s)}"
+  assumes \<open>is_axiom (list_sequent s)\<close>
+  shows \<open>calculation s = {(0,s)}\<close>
 proof (rule set_eqI,simp add: split_paired_all)
   fix n k
-  show "((n,k) \<in> calculation s) = (n = 0 \<and> k = s)"
+  show \<open>((n,k) \<in> calculation s) = (n = 0 \<and> k = s)\<close>
   proof (rule iffI)
-    assume "(n,k) \<in> calculation s" then show "(n = 0 \<and> k = s)"
+    assume \<open>(n,k) \<in> calculation s\<close> then show \<open>(n = 0 \<and> k = s)\<close>
       using assms calculation.simps calculation_calculation_child by metis
   next
-    assume "(n = 0 \<and> k = s)" then show "(n,k) \<in> calculation s"
+    assume \<open>(n = 0 \<and> k = s)\<close> then show \<open>(n,k) \<in> calculation s\<close>
       using assms calculation.simps by blast
   qed
 qed
 
-lemma is_axiom_finite_calculation: "is_axiom (list_sequent s) \<Longrightarrow> finite (calculation s)"
-by (simp add: calculation_is_axiom)
+lemma is_axiom_finite_calculation: \<open>is_axiom (list_sequent s) \<Longrightarrow> finite (calculation s)\<close>
+  by (simp add: calculation_is_axiom)
 
-primrec failing_path :: "(nat \<times> sequent) set \<Rightarrow> nat \<Rightarrow> (nat \<times> sequent)" where
-  "failing_path ns 0 = (SOME x. x \<in> ns \<and> fst x = 0 \<and> infinite (calculation (snd x)) \<and>
-    \<not> is_axiom (list_sequent (snd x)))" |
-  "failing_path ns (Suc n) = (let fn = failing_path ns n in
+primrec failing_path :: \<open>(nat \<times> sequent) set \<Rightarrow> nat \<Rightarrow> (nat \<times> sequent)\<close> where
+  \<open>failing_path ns 0 = (SOME x. x \<in> ns \<and> fst x = 0 \<and> infinite (calculation (snd x)) \<and>
+    \<not> is_axiom (list_sequent (snd x)))\<close> |
+  \<open>failing_path ns (Suc n) = (let fn = failing_path ns n in
     (SOME fsucn. fsucn \<in> ns \<and> fst fsucn = Suc n \<and> (snd fsucn) \<in> set (solve (snd fn)) \<and>
-      infinite (calculation (snd fsucn)) \<and> \<not> is_axiom (list_sequent (snd fsucn))))"
+      infinite (calculation (snd fsucn)) \<and> \<not> is_axiom (list_sequent (snd fsucn))))\<close>
 
 lemma f0:
-  assumes "f = failing_path (calculation s)"
-  and "infinite (calculation s)"
-  shows "f 0 \<in> (calculation s) \<and> fst (f 0) = 0 \<and> infinite (calculation (snd (f 0))) \<and>
-    \<not> is_axiom (list_sequent (snd (f 0)))"
+  assumes \<open>f = failing_path (calculation s)\<close>
+    and \<open>infinite (calculation s)\<close>
+  shows \<open>f 0 \<in> (calculation s) \<and> fst (f 0) = 0 \<and> infinite (calculation (snd (f 0))) \<and>
+    \<not> is_axiom (list_sequent (snd (f 0)))\<close>
 proof -
-  have "\<And>p P. p \<notin> P \<or> fst p \<noteq> (0::nat) \<or> finite (calculation (snd p)) \<or>
+  have \<open>\<And>p P. p \<notin> P \<or> fst p \<noteq> (0::nat) \<or> finite (calculation (snd p)) \<or>
     (SOME p. p \<in> P \<and> fst p = 0 \<and> infinite (calculation (snd p)) \<and>
       \<not> is_axiom (list_sequent (snd p))) \<in> P \<and> fst (SOME p. p \<in> P \<and> fst p = 0 \<and>
       infinite (calculation (snd p)) \<and> \<not> is_axiom (list_sequent (snd p))) = 0 \<and>
       infinite (calculation (snd (SOME p. p \<in> P \<and> fst p = 0 \<and>
       infinite (calculation (snd p)) \<and> \<not> is_axiom (list_sequent (snd p))))) \<and>
       \<not> is_axiom (list_sequent (snd (SOME p. p \<in> P \<and> fst p = 0 \<and>
-      infinite (calculation (snd p)) \<and> \<not> is_axiom (list_sequent (snd p)))))"
+      infinite (calculation (snd p)) \<and> \<not> is_axiom (list_sequent (snd p)))))\<close>
   proof -
-    fix p :: "nat \<times> (nat \<times> nnf) list" and P :: "(nat \<times> (nat \<times> nnf) list) set"
-    have f1: "\<forall>p pa. \<not> p (pa::nat \<times> (nat \<times> nnf) list) \<or> p (Eps p)" by (metis someI)
-    { assume "(SOME p. p \<in> P \<and> fst p = 0 \<and> infinite (calculation (snd p)) \<and>
+    fix p :: \<open>nat \<times> (nat \<times> nnf) list\<close> and P :: \<open>(nat \<times> (nat \<times> nnf) list) set\<close>
+    have f1: \<open>\<forall>p pa. \<not> p (pa::nat \<times> (nat \<times> nnf) list) \<or> p (Eps p)\<close> by (metis someI)
+    { assume \<open>(SOME p. p \<in> P \<and> fst p = 0 \<and> infinite (calculation (snd p)) \<and>
       \<not> is_axiom (list_sequent (snd p))) \<notin> P \<or> fst (SOME p. p \<in> P \<and> fst p = 0 \<and>
       infinite (calculation (snd p)) \<and> \<not> is_axiom (list_sequent (snd p))) \<noteq> 0 \<or>
       finite (calculation (snd (SOME p. p \<in> P \<and> fst p = 0 \<and> infinite (calculation (snd p)) \<and>
       \<not> is_axiom (list_sequent (snd p))))) \<or> is_axiom (list_sequent (snd (SOME p. p \<in> P \<and>
-      fst p = 0 \<and> infinite (calculation (snd p)) \<and> \<not> is_axiom (list_sequent (snd p)))))"
-      then have "\<not> ((SOME p. p \<in> P \<and> fst p = 0 \<and> infinite (calculation (snd p)) \<and>
+      fst p = 0 \<and> infinite (calculation (snd p)) \<and> \<not> is_axiom (list_sequent (snd p)))))\<close>
+      then have \<open>\<not> ((SOME p. p \<in> P \<and> fst p = 0 \<and> infinite (calculation (snd p)) \<and>
         \<not> is_axiom (list_sequent (snd p))) \<in> P \<and> fst (SOME p. p \<in> P \<and> fst p = 0 \<and>
         infinite (calculation (snd p)) \<and> \<not> is_axiom (list_sequent (snd p))) = 0 \<and>
         infinite (calculation (snd (SOME p. p \<in> P \<and> fst p = 0 \<and>
         infinite (calculation (snd p)) \<and> \<not> is_axiom (list_sequent (snd p))))) \<and>
         \<not> is_axiom (list_sequent (snd (SOME p. p \<in> P \<and> fst p = 0 \<and>
-        infinite (calculation (snd p)) \<and> \<not> is_axiom (list_sequent (snd p))))))"
+        infinite (calculation (snd p)) \<and> \<not> is_axiom (list_sequent (snd p))))))\<close>
         by metis
-      then have "\<not> (p \<in> P \<and> fst p = 0 \<and> infinite (calculation (snd p)) \<and>
-        \<not> is_axiom (list_sequent (snd p)))"
+      then have \<open>\<not> (p \<in> P \<and> fst p = 0 \<and> infinite (calculation (snd p)) \<and>
+        \<not> is_axiom (list_sequent (snd p)))\<close>
         using f1 by (metis (mono_tags, lifting) someI)
-      then have "p \<notin> P \<or> fst p \<noteq> 0 \<or> finite (calculation (snd p)) \<or>
+      then have \<open>p \<notin> P \<or> fst p \<noteq> 0 \<or> finite (calculation (snd p)) \<or>
         (SOME p. p \<in> P \<and> fst p = 0 \<and> infinite (calculation (snd p)) \<and>
         \<not> is_axiom (list_sequent (snd p))) \<in> P \<and> fst (SOME p. p \<in> P \<and> fst p = 0 \<and>
         infinite (calculation (snd p)) \<and> \<not> is_axiom (list_sequent (snd p))) = 0 \<and>
         infinite (calculation (snd (SOME p. p \<in> P \<and> fst p = 0 \<and>
         infinite (calculation (snd p)) \<and> \<not> is_axiom (list_sequent (snd p))))) \<and>
         \<not> is_axiom (list_sequent (snd (SOME p. p \<in> P \<and> fst p = 0 \<and>
-        infinite (calculation (snd p)) \<and> \<not> is_axiom (list_sequent (snd p)))))"
+        infinite (calculation (snd p)) \<and> \<not> is_axiom (list_sequent (snd p)))))\<close>
         by (metis (no_types) is_axiom_finite_calculation) }
-     then show "p \<notin> P \<or> fst p \<noteq> 0 \<or> finite (calculation (snd p)) \<or>
+    then show \<open>p \<notin> P \<or> fst p \<noteq> 0 \<or> finite (calculation (snd p)) \<or>
        (SOME p. p \<in> P \<and> fst p = 0 \<and> infinite (calculation (snd p)) \<and>
        \<not> is_axiom (list_sequent (snd p))) \<in> P \<and> fst (SOME p. p \<in> P \<and> fst p = 0 \<and>
        infinite (calculation (snd p)) \<and> \<not> is_axiom (list_sequent (snd p))) = 0 \<and>
        infinite (calculation (snd (SOME p. p \<in> P \<and> fst p = 0 \<and>
        infinite (calculation (snd p)) \<and> \<not> is_axiom (list_sequent (snd p))))) \<and>
        \<not> is_axiom (list_sequent (snd (SOME p. p \<in> P \<and> fst p = 0 \<and>
-       infinite (calculation (snd p)) \<and> \<not> is_axiom (list_sequent (snd p)))))"
-       by blast
+       infinite (calculation (snd p)) \<and> \<not> is_axiom (list_sequent (snd p)))))\<close>
+      by blast
   qed
-  then have "\<And>ps. fst (0::nat, ps) \<noteq> 0 \<or> finite (calculation (snd (0::nat, ps))) \<or>
+  then have \<open>\<And>ps. fst (0::nat, ps) \<noteq> 0 \<or> finite (calculation (snd (0::nat, ps))) \<or>
     (SOME p. p \<in> calculation ps \<and> fst p = 0 \<and> infinite (calculation (snd p)) \<and>
     \<not> is_axiom (list_sequent (snd p))) \<in> calculation ps \<and>
     fst (SOME p. p \<in> calculation ps \<and> fst p = 0 \<and>
@@ -833,129 +835,129 @@ proof -
     infinite (calculation (snd (SOME p. p \<in> calculation ps \<and> fst p = 0 \<and>
     infinite (calculation (snd p)) \<and> \<not> is_axiom (list_sequent (snd p))))) \<and>
     \<not> is_axiom (list_sequent (snd (SOME p. p \<in> calculation ps \<and> fst p = 0 \<and>
-    infinite (calculation (snd p)) \<and> \<not> is_axiom (list_sequent (snd p)))))"
+    infinite (calculation (snd p)) \<and> \<not> is_axiom (list_sequent (snd p)))))\<close>
     by (meson calculation.simps)
   then show ?thesis
     using assms(1) assms(2) by auto
 qed
 
-lemma infinite_union: "finite Y \<Longrightarrow> infinite (Union (f ` Y)) \<Longrightarrow> \<exists>y. y \<in> Y \<and> infinite (f y)"
-by auto
+lemma infinite_union: \<open>finite Y \<Longrightarrow> infinite (Union (f ` Y)) \<Longrightarrow> \<exists>y. y \<in> Y \<and> infinite (f y)\<close>
+  by auto
 
-lemma finite_subs: "finite {w. \<not> is_axiom (list_sequent y) \<and> w \<in> set (solve y)}"
-by simp
+lemma finite_subs: \<open>finite {w. \<not> is_axiom (list_sequent y) \<and> w \<in> set (solve y)}\<close>
+  by simp
 
 lemma fSuc:
-  assumes "f = failing_path (calculation s)"
-  and "f n \<in> calculation s \<and> fst (f n) = n \<and> infinite (calculation (snd (f n))) \<and>
-    \<not> is_axiom (list_sequent (snd (f n)))"
-  shows "f (Suc n) \<in> calculation s \<and> fst (f (Suc n)) = Suc n \<and> (snd (f (Suc n)))
+  assumes \<open>f = failing_path (calculation s)\<close>
+    and \<open>f n \<in> calculation s \<and> fst (f n) = n \<and> infinite (calculation (snd (f n))) \<and>
+    \<not> is_axiom (list_sequent (snd (f n)))\<close>
+  shows \<open>f (Suc n) \<in> calculation s \<and> fst (f (Suc n)) = Suc n \<and> (snd (f (Suc n)))
     \<in> set (solve (snd (f n))) \<and> infinite (calculation (snd (f (Suc n)))) \<and>
-    \<not> is_axiom (list_sequent (snd (f (Suc n))))"
+    \<not> is_axiom (list_sequent (snd (f (Suc n))))\<close>
 proof -
-  have "infinite (\<Union> (calculation ` {w. \<not> is_axiom (list_sequent (snd (f n))) \<and>
-    w \<in> set (solve (snd (f n)))}))"
+  have \<open>infinite (\<Union> (calculation ` {w. \<not> is_axiom (list_sequent (snd (f n))) \<and>
+    w \<in> set (solve (snd (f n)))}))\<close>
     using assms
     by (metis (mono_tags,lifting) Collect_cong calculation finite.insertI finite_imageI)
   then show ?thesis using assms calculation.intros(2) is_axiom_finite_calculation
     by simp (rule someI_ex,simp,metis prod.collapse)
 qed
 
-lemma is_path_f_0: "infinite (calculation s) \<Longrightarrow> failing_path (calculation s) 0 = (0,s)"
-using calculation_init f0 prod.collapse
-by metis
+lemma is_path_f_0: \<open>infinite (calculation s) \<Longrightarrow> failing_path (calculation s) 0 = (0,s)\<close>
+  using calculation_init f0 prod.collapse
+  by metis
 
 lemma is_path_f':
-  assumes "f = failing_path (calculation s)"
-  and "infinite (calculation s)"
-  shows "f n \<in> calculation s \<and> fst (f n) = n \<and> infinite (calculation (snd (f n))) \<and>
-    \<not> is_axiom (list_sequent (snd (f n)))"
-using assms f0 fSuc
-by (induct n) simp_all
+  assumes \<open>f = failing_path (calculation s)\<close>
+    and \<open>infinite (calculation s)\<close>
+  shows \<open>f n \<in> calculation s \<and> fst (f n) = n \<and> infinite (calculation (snd (f n))) \<and>
+    \<not> is_axiom (list_sequent (snd (f n)))\<close>
+  using assms f0 fSuc
+  by (induct n) simp_all
 
 lemma is_path_f:
-  assumes "f = failing_path (calculation s)"
-  and "infinite (calculation s)"
-  shows "\<forall>n. f n \<in> calculation s \<and> fst (f n) = n \<and> (snd (f (Suc n))) \<in> set (solve (snd (f n))) \<and>
-    infinite (calculation (snd (f n)))"
-using assms is_path_f' fSuc
-by simp
+  assumes \<open>f = failing_path (calculation s)\<close>
+    and \<open>infinite (calculation s)\<close>
+  shows \<open>\<forall>n. f n \<in> calculation s \<and> fst (f n) = n \<and> (snd (f (Suc n))) \<in> set (solve (snd (f n))) \<and>
+    infinite (calculation (snd (f n)))\<close>
+  using assms is_path_f' fSuc
+  by simp
 
-lemma dump: "Suc n \<in> set l = (n \<in> set (dump l))"
+lemma dump: \<open>Suc n \<in> set l = (n \<in> set (dump l))\<close>
 proof (induct l)
   case Nil then show ?case by simp
 next
   case (Cons m _) then show ?case by (cases m) simp_all
 qed
 
-lemma ts0: "(\<And>e e'. \<forall>x. x \<in> set (free p) \<longrightarrow> e x = e' x \<Longrightarrow> semantics m e p = semantics m e' p)
+lemma ts0: \<open>(\<And>e e'. \<forall>x. x \<in> set (free p) \<longrightarrow> e x = e' x \<Longrightarrow> semantics m e p = semantics m e' p)
   \<Longrightarrow> \<forall>x. x \<in> set (dump (free p)) \<longrightarrow> e x = e' x \<Longrightarrow>
   (\<forall>z\<in>fst m. semantics m (\<lambda>x. case x of 0 \<Rightarrow> z | Suc n \<Rightarrow> e n) p) =
-    (\<forall>z\<in>fst m. semantics m (\<lambda>x. case x of 0 \<Rightarrow> z | Suc n \<Rightarrow> e' n) p)"
+    (\<forall>z\<in>fst m. semantics m (\<lambda>x. case x of 0 \<Rightarrow> z | Suc n \<Rightarrow> e' n) p)\<close>
 proof -
-  assume a1: "\<And>e e'. \<forall>x. x \<in> set (free p) \<longrightarrow> e x = e' x \<Longrightarrow> semantics m e p = semantics m e' p"
-  assume a2: "\<forall>x. x \<in> set (dump (free p)) \<longrightarrow> e x = e' x"
-  have f3: "((\<forall>us. us \<in> fst m \<longrightarrow> semantics m (case_nat us e) p) \<noteq> (\<forall>us. us \<in> fst m \<longrightarrow>
+  assume a1: \<open>\<And>e e'. \<forall>x. x \<in> set (free p) \<longrightarrow> e x = e' x \<Longrightarrow> semantics m e p = semantics m e' p\<close>
+  assume a2: \<open>\<forall>x. x \<in> set (dump (free p)) \<longrightarrow> e x = e' x\<close>
+  have f3: \<open>((\<forall>us. us \<in> fst m \<longrightarrow> semantics m (case_nat us e) p) \<noteq> (\<forall>us. us \<in> fst m \<longrightarrow>
     semantics m (case_nat us e') p)) = ((\<exists>us. us \<in> fst m \<and>
-    \<not> semantics m (case_nat us e) p) = (\<forall>us. us \<notin> fst m \<or> semantics m (case_nat us e') p))"
+    \<not> semantics m (case_nat us e) p) = (\<forall>us. us \<notin> fst m \<or> semantics m (case_nat us e') p))\<close>
     by blast
   obtain uus and uusa where
-    f4: "((\<exists>us. us \<in> fst m \<and> \<not> semantics m (case_nat us e) p) =
+    f4: \<open>((\<exists>us. us \<in> fst m \<and> \<not> semantics m (case_nat us e) p) =
       (\<forall>us. us \<notin> fst m \<or> semantics m (case_nat us e') p)) =
       (((\<forall>us. us \<notin> fst m \<or> semantics m (case_nat us e) p) \<or>
         (\<forall>us. us \<notin> fst m \<or> semantics m (case_nat us e') p)) \<and>
         (uusa \<in> fst m \<and> \<not> semantics m (case_nat uusa e) p \<or> uus \<in> fst m \<and>
-        \<not> semantics m (case_nat uus e') p))"
+        \<not> semantics m (case_nat uus e') p))\<close>
     by (metis (no_types))
-  then have "(\<exists>us. us \<in> fst m \<and> \<not> semantics m (case_nat us e) p) \<and>
+  then have \<open>(\<exists>us. us \<in> fst m \<and> \<not> semantics m (case_nat us e) p) \<and>
     (\<exists>us. us \<in> fst m \<and> \<not> semantics m (case_nat us e') p) \<or>
     (uusa \<notin> fst m \<or> semantics m (case_nat uusa e) p) \<and> (uus \<notin> fst m \<or>
-    semantics m (case_nat uus e') p)"
+    semantics m (case_nat uus e') p)\<close>
     using a2 a1 by (metis (no_types,lifting) Nitpick.case_nat_unfold Suc_pred' dump neq0_conv)
-  then have "(\<forall>us. us \<in> fst m \<longrightarrow> semantics m (case_nat us e) p) =
-    (\<forall>us. us \<in> fst m \<longrightarrow> semantics m (case_nat us e') p)"
+  then have \<open>(\<forall>us. us \<in> fst m \<longrightarrow> semantics m (case_nat us e) p) =
+    (\<forall>us. us \<in> fst m \<longrightarrow> semantics m (case_nat us e') p)\<close>
     using f4 f3 by blast
   then show ?thesis
     by blast
 qed
 
-lemma ts1: "(\<And>e e'. \<forall>x. x \<in> set (free p) \<longrightarrow> e x = e' x \<Longrightarrow> semantics m e p = semantics m e' p)
+lemma ts1: \<open>(\<And>e e'. \<forall>x. x \<in> set (free p) \<longrightarrow> e x = e' x \<Longrightarrow> semantics m e p = semantics m e' p)
   \<Longrightarrow> \<forall>x. x \<in> set (dump (free p)) \<longrightarrow> e x = e' x \<Longrightarrow>
   (\<exists>z\<in>fst m. semantics m (\<lambda>x. case x of 0 \<Rightarrow> z | Suc n \<Rightarrow> e n) p) =
-    (\<exists>z\<in>fst m. semantics m (\<lambda>x. case x of 0 \<Rightarrow> z | Suc n \<Rightarrow> e' n) p)"
+    (\<exists>z\<in>fst m. semantics m (\<lambda>x. case x of 0 \<Rightarrow> z | Suc n \<Rightarrow> e' n) p)\<close>
 proof -
-  assume a1: "\<And>e e'. \<forall>x. x \<in> set (free p) \<longrightarrow> e x = e' x \<Longrightarrow> semantics m e p = semantics m e' p"
-  assume a2: "\<forall>x. x \<in> set (dump (free p)) \<longrightarrow> e x = e' x"
-  have f3: "\<forall>us f n. if n = 0 then (case n of 0 \<Rightarrow> us::unit list | Suc x \<Rightarrow> f x) =
-    us else (case n of 0 \<Rightarrow> us | Suc x \<Rightarrow> f x) = f (n - 1)"
+  assume a1: \<open>\<And>e e'. \<forall>x. x \<in> set (free p) \<longrightarrow> e x = e' x \<Longrightarrow> semantics m e p = semantics m e' p\<close>
+  assume a2: \<open>\<forall>x. x \<in> set (dump (free p)) \<longrightarrow> e x = e' x\<close>
+  have f3: \<open>\<forall>us f n. if n = 0 then (case n of 0 \<Rightarrow> us::unit list | Suc x \<Rightarrow> f x) =
+    us else (case n of 0 \<Rightarrow> us | Suc x \<Rightarrow> f x) = f (n - 1)\<close>
     by (simp add: Nitpick.case_nat_unfold)
   obtain uus and uusa where
-    f4: "((\<forall>us. us \<notin> fst m \<or> \<not> semantics m (case_nat us e) p) =
+    f4: \<open>((\<forall>us. us \<notin> fst m \<or> \<not> semantics m (case_nat us e) p) =
       (\<exists>us. us \<in> fst m \<and> semantics m (case_nat us e') p)) =
       ((uusa \<in> fst m \<and> semantics m (case_nat uusa e) p \<or> uus \<in> fst m \<and>
       semantics m (case_nat uus e') p) \<and> ((\<forall>us. us \<notin> fst m \<or> \<not> semantics m (case_nat us e) p) \<or>
-      (\<forall>us. us \<notin> fst m \<or> \<not> semantics m (case_nat us e') p)))"
+      (\<forall>us. us \<notin> fst m \<or> \<not> semantics m (case_nat us e') p)))\<close>
     by blast
-  have "(uusa \<notin> fst m \<or> \<not> semantics m (case_nat uusa e) p) \<and> (uus \<notin> fst m \<or>
+  have \<open>(uusa \<notin> fst m \<or> \<not> semantics m (case_nat uusa e) p) \<and> (uus \<notin> fst m \<or>
     \<not> semantics m (case_nat uus e') p) \<or> (\<exists>us. us \<in> fst m \<and> semantics m (case_nat us e) p) \<and>
-      (\<exists>us. us \<in> fst m \<and> semantics m (case_nat us e') p)"
+      (\<exists>us. us \<in> fst m \<and> semantics m (case_nat us e') p)\<close>
     using f3 a2 a1
-    proof -
-      obtain nn :: "(nat \<Rightarrow> proxy) \<Rightarrow> (nat \<Rightarrow> proxy) \<Rightarrow> nat" where
-        f1: "\<forall>f fa. nn fa f \<in> set (free p) \<and> f (nn fa f) \<noteq> fa (nn fa f) \<or>
-          semantics m f p = semantics m fa p"
-        using a1 by moura
-      have "\<forall>p f n. if n = 0 then (case n of 0 \<Rightarrow> p::proxy | Suc x \<Rightarrow> f x) = p else
-        (case n of 0 \<Rightarrow> p | Suc x \<Rightarrow> f x) = f (n - 1)"
-        by (simp add: Nitpick.case_nat_unfold)
-      then show ?thesis
-        using f1 by (metis (no_types) Suc_pred' a2 dump not_gr0)
-    qed
+  proof -
+    obtain nn :: \<open>(nat \<Rightarrow> proxy) \<Rightarrow> (nat \<Rightarrow> proxy) \<Rightarrow> nat\<close> where
+      f1: \<open>\<forall>f fa. nn fa f \<in> set (free p) \<and> f (nn fa f) \<noteq> fa (nn fa f) \<or>
+          semantics m f p = semantics m fa p\<close>
+      using a1 by moura
+    have \<open>\<forall>p f n. if n = 0 then (case n of 0 \<Rightarrow> p::proxy | Suc x \<Rightarrow> f x) = p else
+        (case n of 0 \<Rightarrow> p | Suc x \<Rightarrow> f x) = f (n - 1)\<close>
+      by (simp add: Nitpick.case_nat_unfold)
+    then show ?thesis
+      using f1 by (metis (no_types) Suc_pred' a2 dump not_gr0)
+  qed
   then show ?thesis
     using f4 by blast
 qed
 
-lemma eval_cong: "\<forall>x. x \<in> set (free p) \<longrightarrow> e x = e' x \<Longrightarrow> semantics m e p = semantics m e' p"
+lemma eval_cong: \<open>\<forall>x. x \<in> set (free p) \<longrightarrow> e x = e' x \<Longrightarrow> semantics m e p = semantics m e' p\<close>
 proof (induct p arbitrary: e e')
   case Pre then show ?case using map_cong free.simps(1) semantics.simps(1) by metis
 next
@@ -968,134 +970,134 @@ next
   case Exi then show ?case using ts1 by simp
 qed
 
-lemma semantics_alternative_def2: "semantics_alternative m e s = (\<exists>p. p \<in> set s \<and> semantics m e p)"
-by (induct s) auto
+lemma semantics_alternative_def2: \<open>semantics_alternative m e s = (\<exists>p. p \<in> set s \<and> semantics m e p)\<close>
+  by (induct s) auto
 
-lemma semantics_alternative_append: "semantics_alternative m e (s @ s') =
-  ((semantics_alternative m e s) \<or> (semantics_alternative m e s'))"
-by (induct s) auto
+lemma semantics_alternative_append: \<open>semantics_alternative m e (s @ s') =
+  ((semantics_alternative m e s) \<or> (semantics_alternative m e s'))\<close>
+  by (induct s) auto
 
-lemma fv_list_cons: "fv_list (a # list) = (free a) @ (fv_list list)"
-by (simp add: fv_list_def maps)
+lemma fv_list_cons: \<open>fv_list (a # list) = (free a) @ (fv_list list)\<close>
+  by (simp add: fv_list_def maps)
 
-lemma semantics_alternative_cong: "(\<forall>x. x \<in> set (fv_list s) \<longrightarrow> e x = e' x) \<longrightarrow>
-  semantics_alternative m e s = semantics_alternative m e' s"
-by (induct s) (simp_all,metis eval_cong Un_iff set_append fv_list_cons)
+lemma semantics_alternative_cong: \<open>(\<forall>x. x \<in> set (fv_list s) \<longrightarrow> e x = e' x) \<longrightarrow>
+  semantics_alternative m e s = semantics_alternative m e' s\<close>
+  by (induct s) (simp_all,metis eval_cong Un_iff set_append fv_list_cons)
 
-subsection "Soundness"
+subsection \<open>Soundness\<close>
 
-lemma ball: "\<forall>x \<in> m. P x = Q x \<Longrightarrow> (\<exists>x \<in> m. P x) = (\<exists>x \<in> m. Q x)"
-by simp_all
+lemma ball: \<open>\<forall>x \<in> m. P x = Q x \<Longrightarrow> (\<exists>x \<in> m. P x) = (\<exists>x \<in> m. Q x)\<close>
+  by simp_all
 
-definition bump' :: "(nat \<Rightarrow> nat) \<Rightarrow> nat \<Rightarrow> nat" where
-  "bump' f x \<equiv> (case x of 0 \<Rightarrow> 0 | Suc n \<Rightarrow> Suc (f n))"
+definition bump' :: \<open>(nat \<Rightarrow> nat) \<Rightarrow> nat \<Rightarrow> nat\<close> where
+  \<open>bump' f x \<equiv> (case x of 0 \<Rightarrow> 0 | Suc n \<Rightarrow> Suc (f n))\<close>
 
-lemma bump': "increase f x = bump' f x"
-by (metis Nitpick.case_nat_unfold increase.simps Suc_pred' bump'_def not_gr0)
+lemma bump': \<open>increase f x = bump' f x\<close>
+  by (metis Nitpick.case_nat_unfold increase.simps Suc_pred' bump'_def not_gr0)
 
-lemma s0: "semantics m e (sv f p) = semantics m (e \<circ> f) p \<Longrightarrow>
+lemma s0: \<open>semantics m e (sv f p) = semantics m (e \<circ> f) p \<Longrightarrow>
   (\<And>p e e' m. \<forall>x. x \<in> set (free p) \<longrightarrow> e x = e' x \<Longrightarrow> semantics m e p = semantics m e' p) \<Longrightarrow>
   (\<forall>z\<in>fst m. semantics m (case_nat z e \<circ> increase f) p) =
-    (\<forall>z\<in>fst m. semantics m (\<lambda>x. case x of 0 \<Rightarrow> z | Suc n \<Rightarrow> (e \<circ> f) n) p)"
+    (\<forall>z\<in>fst m. semantics m (\<lambda>x. case x of 0 \<Rightarrow> z | Suc n \<Rightarrow> (e \<circ> f) n) p)\<close>
 proof -
-  assume a1: "\<And>p e e' m. \<forall>x. x \<in> set (free p) \<longrightarrow>
-              e x = e' x \<Longrightarrow> semantics m e p = semantics m e' p"
+  assume a1: \<open>\<And>p e e' m. \<forall>x. x \<in> set (free p) \<longrightarrow>
+              e x = e' x \<Longrightarrow> semantics m e p = semantics m e' p\<close>
   obtain q :: proxy and a :: proxy where
-    f2: "((\<exists>pa. pa \<in> fst m \<and> \<not> semantics m (case_nat pa e \<circ> increase f) p) = (\<forall>pa. pa \<notin> fst m \<or>
+    f2: \<open>((\<exists>pa. pa \<in> fst m \<and> \<not> semantics m (case_nat pa e \<circ> increase f) p) = (\<forall>pa. pa \<notin> fst m \<or>
       semantics m (case_nat pa (e \<circ> f)) p)) = (((\<forall>pa. pa \<notin> fst m \<or> semantics m (case_nat pa e \<circ>
       increase f) p) \<or> (\<forall>pa. pa \<notin> fst m \<or> semantics m (case_nat pa (e \<circ> f)) p)) \<and> (a \<in> fst m \<and>
       \<not> semantics m (case_nat a e \<circ> increase f) p \<or> q \<in> fst m \<and>
-      \<not> semantics m (case_nat q (e \<circ> f)) p))"
+      \<not> semantics m (case_nat q (e \<circ> f)) p))\<close>
     by moura
-  have f3: "\<forall>n f fa p. (\<exists>na. na \<in> set (free n) \<and> f na \<noteq> fa na)
-           \<or> semantics p f n = semantics p fa n"
+  have f3: \<open>\<forall>n f fa p. (\<exists>na. na \<in> set (free n) \<and> f na \<noteq> fa na)
+           \<or> semantics p f n = semantics p fa n\<close>
     using a1 by (metis (no_types))
-  obtain nn :: "(nat \<Rightarrow> proxy) \<Rightarrow> (nat \<Rightarrow> proxy) \<Rightarrow> nnf \<Rightarrow> nat" where
-    "\<forall>x1 x2 x3. (\<exists>v4. v4 \<in> set (free x3) \<and> x2 v4 \<noteq> x1 v4) = (nn x1 x2 x3 \<in> set (free x3) \<and> x2
-      (nn x1 x2 x3) \<noteq> x1 (nn x1 x2 x3))"
+  obtain nn :: \<open>(nat \<Rightarrow> proxy) \<Rightarrow> (nat \<Rightarrow> proxy) \<Rightarrow> nnf \<Rightarrow> nat\<close> where
+    \<open>\<forall>x1 x2 x3. (\<exists>v4. v4 \<in> set (free x3) \<and> x2 v4 \<noteq> x1 v4) = (nn x1 x2 x3 \<in> set (free x3) \<and> x2
+      (nn x1 x2 x3) \<noteq> x1 (nn x1 x2 x3))\<close>
     by moura
-  then have f4: "\<forall>n f fa p. nn fa f n \<in> set (free n) \<and> f (nn fa f n) \<noteq> fa (nn fa f n) \<or>
-      semantics p f n = semantics p fa n"
+  then have f4: \<open>\<forall>n f fa p. nn fa f n \<in> set (free n) \<and> f (nn fa f n) \<noteq> fa (nn fa f n) \<or>
+      semantics p f n = semantics p fa n\<close>
     using f3 by presburger
-  have f5: "\<forall>p f n. if n = 0 then (case n of 0 \<Rightarrow> p::proxy | Suc x \<Rightarrow> f x) = p else
-    (case n of 0 \<Rightarrow> p | Suc x \<Rightarrow> f x) = f (n - 1)"
+  have f5: \<open>\<forall>p f n. if n = 0 then (case n of 0 \<Rightarrow> p::proxy | Suc x \<Rightarrow> f x) = p else
+    (case n of 0 \<Rightarrow> p | Suc x \<Rightarrow> f x) = f (n - 1)\<close>
     by (metis (no_types) Nitpick.case_nat_unfold)
-  then have f6: "(case increase f (nn (case_nat a (e \<circ> f)) (case_nat a e \<circ> increase f) p) of 0 \<Rightarrow> a
+  then have f6: \<open>(case increase f (nn (case_nat a (e \<circ> f)) (case_nat a e \<circ> increase f) p) of 0 \<Rightarrow> a
       | Suc x \<Rightarrow> e x) = a \<and> (case_nat a e \<circ> increase f) (nn (case_nat a (e \<circ> f)) (case_nat a e \<circ>
       increase f) p) \<noteq> (case nn (case_nat a (e \<circ> f)) (case_nat a e \<circ> increase f) p of 0 \<Rightarrow> a |
-      Suc x \<Rightarrow> (e \<circ> f) x) \<longrightarrow> nn (case_nat a (e \<circ> f)) (case_nat a e \<circ> increase f) p \<noteq> 0"
+      Suc x \<Rightarrow> (e \<circ> f) x) \<longrightarrow> nn (case_nat a (e \<circ> f)) (case_nat a e \<circ> increase f) p \<noteq> 0\<close>
     by (metis o_apply)
-  have f7: "\<forall>n f na. if na = 0 then (case na of 0 \<Rightarrow> n::nat | Suc x \<Rightarrow> f x) = n else
-    (case na of 0 \<Rightarrow> n | Suc x \<Rightarrow> f x) = f (na - 1)"
+  have f7: \<open>\<forall>n f na. if na = 0 then (case na of 0 \<Rightarrow> n::nat | Suc x \<Rightarrow> f x) = n else
+    (case na of 0 \<Rightarrow> n | Suc x \<Rightarrow> f x) = f (na - 1)\<close>
     by (simp add: Nitpick.case_nat_unfold)
-  have "(case_nat a e \<circ> increase f) (nn (case_nat a (e \<circ> f)) (case_nat a e \<circ> increase f) p) \<noteq>
+  have \<open>(case_nat a e \<circ> increase f) (nn (case_nat a (e \<circ> f)) (case_nat a e \<circ> increase f) p) \<noteq>
     (case nn (case_nat a (e \<circ> f)) (case_nat a e \<circ> increase f) p of 0 \<Rightarrow> a | Suc x \<Rightarrow> (e \<circ> f) x)
-    \<longrightarrow> nn (case_nat a (e \<circ> f)) (case_nat a e \<circ> increase f) p \<noteq> 0"
+    \<longrightarrow> nn (case_nat a (e \<circ> f)) (case_nat a e \<circ> increase f) p \<noteq> 0\<close>
     using f6 bump'_def by fastforce
-  then have f8: "(case_nat a e \<circ> increase f) (nn (case_nat a (e \<circ> f))
+  then have f8: \<open>(case_nat a e \<circ> increase f) (nn (case_nat a (e \<circ> f))
     (case_nat a e \<circ> increase f) p) \<noteq> (case nn (case_nat a (e \<circ> f))
     (case_nat a e \<circ> increase f) p of 0 \<Rightarrow> a | Suc x \<Rightarrow> (e \<circ> f) x)
     \<longrightarrow> (case_nat a e \<circ> increase f) (nn (case_nat a (e \<circ> f)) (case_nat a e \<circ> increase f) p) =
-    (case nn (case_nat a (e \<circ> f)) (case_nat a e \<circ> increase f) p of 0 \<Rightarrow> a | Suc x \<Rightarrow> (e \<circ> f) x)"
+    (case nn (case_nat a (e \<circ> f)) (case_nat a e \<circ> increase f) p of 0 \<Rightarrow> a | Suc x \<Rightarrow> (e \<circ> f) x)\<close>
     using f7 f5 bump'_def bump' by force
-  have f9: "nn (case_nat q (e \<circ> f)) (case_nat q e \<circ> increase f) p \<noteq> 0 \<longrightarrow>
+  have f9: \<open>nn (case_nat q (e \<circ> f)) (case_nat q e \<circ> increase f) p \<noteq> 0 \<longrightarrow>
     (case_nat q e \<circ> increase f)
     (nn (case_nat q (e \<circ> f)) (case_nat q e \<circ> increase f) p) = (case nn (case_nat q (e \<circ> f))
-    (case_nat q e \<circ> increase f) p of 0 \<Rightarrow> q | Suc x \<Rightarrow> (e \<circ> f) x)"
+    (case_nat q e \<circ> increase f) p of 0 \<Rightarrow> q | Suc x \<Rightarrow> (e \<circ> f) x)\<close>
     using f7 f5 by (simp add: bump'_def bump')
-  then have "(case_nat q e \<circ> increase f) (nn (case_nat q (e \<circ> f)) (case_nat q e \<circ> increase f) p) \<noteq>
+  then have \<open>(case_nat q e \<circ> increase f) (nn (case_nat q (e \<circ> f)) (case_nat q e \<circ> increase f) p) \<noteq>
     (case nn (case_nat q (e \<circ> f)) (case_nat q e \<circ> increase f) p of 0 \<Rightarrow> q | Suc x \<Rightarrow> (e \<circ> f) x) \<longrightarrow>
-    increase f (nn (case_nat q (e \<circ> f)) (case_nat q e \<circ> increase f) p) = 0"
+    increase f (nn (case_nat q (e \<circ> f)) (case_nat q e \<circ> increase f) p) = 0\<close>
     using f7 by (metis bump' bump'_def)
-  then have "(case_nat q e \<circ> increase f) (nn (case_nat q (e \<circ> f)) (case_nat q e \<circ> increase f) p) =
-    (case nn (case_nat q (e \<circ> f)) (case_nat q e \<circ> increase f) p of 0 \<Rightarrow> q | Suc x \<Rightarrow> (e \<circ> f) x)"
+  then have \<open>(case_nat q e \<circ> increase f) (nn (case_nat q (e \<circ> f)) (case_nat q e \<circ> increase f) p) =
+    (case nn (case_nat q (e \<circ> f)) (case_nat q e \<circ> increase f) p of 0 \<Rightarrow> q | Suc x \<Rightarrow> (e \<circ> f) x)\<close>
     using f9 f5 by (metis (no_types) o_apply)
-  then have "(\<exists>pa. pa \<in> fst m \<and> \<not> semantics m (case_nat pa e \<circ> increase f) p) \<and> (\<exists>pa. pa \<in> fst m
+  then have \<open>(\<exists>pa. pa \<in> fst m \<and> \<not> semantics m (case_nat pa e \<circ> increase f) p) \<and> (\<exists>pa. pa \<in> fst m
     \<and> \<not> semantics m (case_nat pa (e \<circ> f)) p) \<or> (a \<notin> fst m \<or>
-    semantics m (case_nat a e \<circ> increase f) p) \<and> (q \<notin> fst m \<or> semantics m (case_nat q (e \<circ> f)) p)"
+    semantics m (case_nat a e \<circ> increase f) p) \<and> (q \<notin> fst m \<or> semantics m (case_nat q (e \<circ> f)) p)\<close>
     using f8 f4 by blast
   then show ?thesis
     using f2 by blast
 qed
 
-lemma eval_subst: "semantics m e (sv f p) = semantics m (e \<circ> f) p"
-by (induct p arbitrary: e f) (simp,simp,simp,
-  simp add: s0 eval_cong,simp add: Nitpick.case_nat_unfold ball bump'_def eval_cong bump')
+lemma eval_subst: \<open>semantics m e (sv f p) = semantics m (e \<circ> f) p\<close>
+  by (induct p arbitrary: e f) (simp,simp,simp,
+      simp add: s0 eval_cong,simp add: Nitpick.case_nat_unfold ball bump'_def eval_cong bump')
 
-definition bind' :: "nat \<Rightarrow> nat \<Rightarrow> nat" where
-  "bind' y x \<equiv> (case x of 0 \<Rightarrow> y | Suc n \<Rightarrow> n)"
+definition bind' :: \<open>nat \<Rightarrow> nat \<Rightarrow> nat\<close> where
+  \<open>bind' y x \<equiv> (case x of 0 \<Rightarrow> y | Suc n \<Rightarrow> n)\<close>
 
-lemma bind': "bind y x = bind' y x"
-by (metis Nitpick.case_nat_unfold bind.simps Suc_pred' bind'_def not_gr0)
+lemma bind': \<open>bind y x = bind' y x\<close>
+  by (metis Nitpick.case_nat_unfold bind.simps Suc_pred' bind'_def not_gr0)
 
-lemma eval_bind: "semantics m e (sv (bind n) p) = semantics m (case_nat (e n) e) p"
-using eval_cong eval_subst
-by (simp add: Nitpick.case_nat_unfold bind'_def bind')
+lemma eval_bind: \<open>semantics m e (sv (bind n) p) = semantics m (case_nat (e n) e) p\<close>
+  using eval_cong eval_subst
+  by (simp add: Nitpick.case_nat_unfold bind'_def bind')
 
 lemma sound_Uni:
-  assumes "u \<notin> set (fv_list (Uni p # s))"
-  and "valid (s@[sv (bind u) p])"
-  shows "valid (Uni p # s)"
+  assumes \<open>u \<notin> set (fv_list (Uni p # s))\<close>
+    and \<open>valid (s@[sv (bind u) p])\<close>
+  shows \<open>valid (Uni p # s)\<close>
 proof (clarsimp simp: valid_def)
   fix M I e z
-  show "is_model_environment (M,I) e \<Longrightarrow> \<not> semantics_alternative (M,I) e s \<Longrightarrow> z \<in> M \<Longrightarrow>
-    semantics (M,I) (case_nat z e) p"
+  show \<open>is_model_environment (M,I) e \<Longrightarrow> \<not> semantics_alternative (M,I) e s \<Longrightarrow> z \<in> M \<Longrightarrow>
+    semantics (M,I) (case_nat z e) p\<close>
   proof -
-    assume zM: "z \<in> M" and sa: "\<not> semantics_alternative (M,I) e s"
-      and ime: "is_model_environment (M,I) e"
-    have 1: "semantics (M,I) (case_nat z (e(u:=z))) p = semantics (M,I) (case_nat z e) p"
+    assume zM: \<open>z \<in> M\<close> and sa: \<open>\<not> semantics_alternative (M,I) e s\<close>
+      and ime: \<open>is_model_environment (M,I) e\<close>
+    have 1: \<open>semantics (M,I) (case_nat z (e(u:=z))) p = semantics (M,I) (case_nat z e) p\<close>
       using assms
       by (clarsimp simp: Nitpick.case_nat_unfold fv_list_cons intro!: eval_cong[rule_format])
         (metis One_nat_def Suc_pred' dump)
-    have "is_model_environment (M,I) (e(u := z)) \<longrightarrow> semantics_alternative (M,I) (e(u := z))
-      (s @ [sv (bind u) p])"
+    have \<open>is_model_environment (M,I) (e(u := z)) \<longrightarrow> semantics_alternative (M,I) (e(u := z))
+      (s @ [sv (bind u) p])\<close>
       using assms valid_def by blast
-    then have 2: "(\<forall>n. (if n = u then z else e n) \<in> M) \<longrightarrow>
-      semantics_alternative (M,I) (e(u := z)) s \<or> semantics (M,I) (case_nat z e) p"
+    then have 2: \<open>(\<forall>n. (if n = u then z else e n) \<in> M) \<longrightarrow>
+      semantics_alternative (M,I) (e(u := z)) s \<or> semantics (M,I) (case_nat z e) p\<close>
       using 1 eval_bind is_model_environment_def semantics_alternative_append by simp
-    have 3: "u \<notin> set (dump (free p)) \<and> u \<notin> set (fv_list s)"
+    have 3: \<open>u \<notin> set (dump (free p)) \<and> u \<notin> set (fv_list s)\<close>
       using assms fv_list_cons by simp
-    have "\<forall>n. e n \<in> M"
+    have \<open>\<forall>n. e n \<in> M\<close>
       using ime is_model_environment_def by simp
     then show ?thesis
       using 2 3 zM sa
@@ -1103,48 +1105,48 @@ proof (clarsimp simp: valid_def)
   qed
 qed
 
-lemma sound_Exi: "valid (s@[sv (bind u) p,Exi p]) \<Longrightarrow> valid (Exi p # s)"
-using valid_def eval_bind
-by (simp add: semantics_alternative_append,metis is_model_environment_def prod.sel(1))
+lemma sound_Exi: \<open>valid (s@[sv (bind u) p,Exi p]) \<Longrightarrow> valid (Exi p # s)\<close>
+  using valid_def eval_bind
+  by (simp add: semantics_alternative_append,metis is_model_environment_def prod.sel(1))
 
-lemma max_exists: "finite (X::nat set) \<Longrightarrow> X \<noteq> {} \<longrightarrow> (\<exists>x. x \<in> X \<and> (\<forall>y. y \<in> X \<longrightarrow> y \<le> x))"
-using Max.coboundedI Max_in
-by blast
+lemma max_exists: \<open>finite (X::nat set) \<Longrightarrow> X \<noteq> {} \<longrightarrow> (\<exists>x. x \<in> X \<and> (\<forall>y. y \<in> X \<longrightarrow> y \<le> x))\<close>
+  using Max.coboundedI Max_in
+  by blast
 
-definition init :: "sequent \<Rightarrow> bool" where
-  "init s == \<forall>x \<in> (set s). fst x = 0"
+definition init :: \<open>sequent \<Rightarrow> bool\<close> where
+  \<open>init s == \<forall>x \<in> (set s). fst x = 0\<close>
 
-definition is_Exi :: "nnf \<Rightarrow> bool" where
-  "is_Exi f \<equiv> case f of Exi _ \<Rightarrow> True | _ \<Rightarrow> False"
+definition is_Exi :: \<open>nnf \<Rightarrow> bool\<close> where
+  \<open>is_Exi f \<equiv> case f of Exi _ \<Rightarrow> True | _ \<Rightarrow> False\<close>
 
-lemma is_Exi: "\<not> is_Exi (Pre b i v) \<and> \<not> is_Exi (Con p q) \<and> \<not> is_Exi (Dis p q) \<and> \<not> is_Exi (Uni p)"
-using is_Exi_def
-by simp
+lemma is_Exi: \<open>\<not> is_Exi (Pre b i v) \<and> \<not> is_Exi (Con p q) \<and> \<not> is_Exi (Dis p q) \<and> \<not> is_Exi (Uni p)\<close>
+  using is_Exi_def
+  by simp
 
 lemma index0:
-  assumes "init s"
-  shows "\<forall>k m p. (n,k) \<in> calculation s \<longrightarrow> (m,p) \<in> (set k) \<longrightarrow> \<not> is_Exi p \<longrightarrow> m = 0"
+  assumes \<open>init s\<close>
+  shows \<open>\<forall>k m p. (n,k) \<in> calculation s \<longrightarrow> (m,p) \<in> (set k) \<longrightarrow> \<not> is_Exi p \<longrightarrow> m = 0\<close>
 proof (induct n)
   case 0 then show ?case using assms init_def calculation_init by fastforce
 next
   case IH: (Suc x)
-    then show ?case
-    proof (intro allI impI)
-      fix k m p
-      show "(Suc x,k) \<in> calculation s \<Longrightarrow> (m,p) \<in> (set k) \<Longrightarrow> \<not> is_Exi p \<Longrightarrow> m = 0"
-      proof -
-        assume "(Suc x,k) \<in> calculation s" and 1: "(m,p) \<in> (set k)" and 2: "\<not> is_Exi p"
-        then obtain t
-          where 3: "(x,t) \<in> calculation s \<and> k \<in> set (solve t) \<and> \<not> is_axiom (list_sequent t)"
-          using calculation_downwards by blast
-        then show ?thesis
-        proof (cases t)
-          case Nil then show ?thesis using assms IH 1 3 by simp
-        next
-         case (Cons a _) then show ?thesis
-         proof (cases a)
+  then show ?case
+  proof (intro allI impI)
+    fix k m p
+    show \<open>(Suc x,k) \<in> calculation s \<Longrightarrow> (m,p) \<in> (set k) \<Longrightarrow> \<not> is_Exi p \<Longrightarrow> m = 0\<close>
+    proof -
+      assume \<open>(Suc x,k) \<in> calculation s\<close> and 1: \<open>(m,p) \<in> (set k)\<close> and 2: \<open>\<not> is_Exi p\<close>
+      then obtain t
+        where 3: \<open>(x,t) \<in> calculation s \<and> k \<in> set (solve t) \<and> \<not> is_axiom (list_sequent t)\<close>
+        using calculation_downwards by blast
+      then show ?thesis
+      proof (cases t)
+        case Nil then show ?thesis using assms IH 1 3 by simp
+      next
+        case (Cons a _) then show ?thesis
+        proof (cases a)
           case (Pair _ q)
-            then show ?thesis using 1 2 3 IH Cons
+          then show ?thesis using 1 2 3 IH Cons
             by (cases q) (fastforce simp: list_sequent_def stop is_Exi_def member_set base)+
         qed
       qed
@@ -1152,178 +1154,178 @@ next
   qed
 qed
 
-lemma maxl: "\<forall>v \<in> set l. v \<le> maxl l"
-by (induct l) (auto simp: max_def mmm)
+lemma maxl: \<open>\<forall>v \<in> set l. v \<le> maxl l\<close>
+  by (induct l) (auto simp: max_def mmm)
 
-lemma fresh: "fresh l \<notin> (set l)"
-unfolding fresh'_def fresh'
-using maxl maxl.simps not_less_eq_eq order_refl empty_iff list.set(1) null.simps(2) list.exhaust
-by metis
+lemma fresh: \<open>fresh l \<notin> (set l)\<close>
+  unfolding fresh'_def fresh'
+  using maxl maxl.simps not_less_eq_eq order_refl empty_iff list.set(1) null.simps(2) list.exhaust
+  by metis
 
 lemma soundness':
-  assumes "init s"
-  and "m \<in> (fst ` (calculation s))"
-  and "\<forall>y u. (y,u) \<in> (calculation s) \<longrightarrow> y \<le> m"
-  shows "\<forall>n t. h = m - n \<and> (n,t) \<in> calculation s \<longrightarrow> valid (list_sequent t)"
+  assumes \<open>init s\<close>
+    and \<open>m \<in> (fst ` (calculation s))\<close>
+    and \<open>\<forall>y u. (y,u) \<in> (calculation s) \<longrightarrow> y \<le> m\<close>
+  shows \<open>\<forall>n t. h = m - n \<and> (n,t) \<in> calculation s \<longrightarrow> valid (list_sequent t)\<close>
 proof (induct h)
   case 0 then show ?case
-    proof (intro allI impI)
-      fix n t
-      show "0 = m - n \<and> (n,t) \<in> calculation s \<Longrightarrow> valid (list_sequent t)"
-      proof -
-        assume *: "0 = m - n \<and> (n,t) \<in> calculation s"
-        then show ?thesis
-        proof (cases "is_axiom (list_sequent t)")
-          case True then show ?thesis
-            proof (cases t)
-              case Nil then show ?thesis using True list_sequent_def by simp
-            next
-              case Cons then show ?thesis
-              using True list_sequent_def valid_def semantics_alternative_def2
-              by simp (metis (no_types,lifting) semantics.simps(1))
-            qed
+  proof (intro allI impI)
+    fix n t
+    show \<open>0 = m - n \<and> (n,t) \<in> calculation s \<Longrightarrow> valid (list_sequent t)\<close>
+    proof -
+      assume *: \<open>0 = m - n \<and> (n,t) \<in> calculation s\<close>
+      then show ?thesis
+      proof (cases \<open>is_axiom (list_sequent t)\<close>)
+        case True then show ?thesis
+        proof (cases t)
+          case Nil then show ?thesis using True list_sequent_def by simp
         next
-          case False
-            then have "n = m" using assms * by fastforce
-            then show ?thesis using assms * False
-            by (meson calculation_upwards le_SucI le_antisym n_not_Suc_n)
+          case Cons then show ?thesis
+            using True list_sequent_def valid_def semantics_alternative_def2
+            by simp (metis (no_types,lifting) semantics.simps(1))
         qed
+      next
+        case False
+        then have \<open>n = m\<close> using assms * by fastforce
+        then show ?thesis using assms * False
+          by (meson calculation_upwards le_SucI le_antisym n_not_Suc_n)
       qed
     qed
+  qed
 next
   case IH: (Suc x) then show ?case
-    proof (intro allI impI)
-      fix n t
-      show "Suc x = m - n \<and> (n,t) \<in> calculation s \<Longrightarrow> valid (list_sequent t)"
-      proof -
-        assume "Suc x = m - n \<and> (n,t) \<in> calculation s"
-        then have *: "Suc x = m - n" and **: "(n,t) \<in> calculation s"
-          by (simp,simp)
-        then show ?thesis
-        proof (cases "is_axiom (list_sequent t)")
-          case True then show ?thesis
-            proof (cases t)
-              case Nil then show ?thesis using True list_sequent_def by simp
-            next
-              case Cons then show ?thesis
-              using True list_sequent_def valid_def semantics_alternative_def2
-              by simp (metis (no_types,lifting) semantics.simps(1))
-            qed
+  proof (intro allI impI)
+    fix n t
+    show \<open>Suc x = m - n \<and> (n,t) \<in> calculation s \<Longrightarrow> valid (list_sequent t)\<close>
+    proof -
+      assume \<open>Suc x = m - n \<and> (n,t) \<in> calculation s\<close>
+      then have *: \<open>Suc x = m - n\<close> and **: \<open>(n,t) \<in> calculation s\<close>
+        by (simp,simp)
+      then show ?thesis
+      proof (cases \<open>is_axiom (list_sequent t)\<close>)
+        case True then show ?thesis
+        proof (cases t)
+          case Nil then show ?thesis using True list_sequent_def by simp
         next
-          case notAxiom: False then show ?thesis
-            proof (cases "\<exists>a f list. t = (a,Uni f) # list")
-              case True
-              then obtain a and f and list where 1: "t = (a,Uni f) # list" by blast
-              then show ?thesis using IH assms * ** fv_list_def fresh list_sequent_def inst_def
-              using instt_def
-              by simp (frule calculation.intros(2),auto simp add: maps instt base frees,
-                  metis (no_types,lifting) Suc_leD diff_Suc_Suc diff_diff_cancel diff_le_self
-                  le_SucI list.map map_append snd_conv sound_Uni)
+          case Cons then show ?thesis
+            using True list_sequent_def valid_def semantics_alternative_def2
+            by simp (metis (no_types,lifting) semantics.simps(1))
+        qed
+      next
+        case notAxiom: False then show ?thesis
+        proof (cases \<open>\<exists>a f list. t = (a,Uni f) # list\<close>)
+          case True
+          then obtain a and f and list where 1: \<open>t = (a,Uni f) # list\<close> by blast
+          then show ?thesis using IH assms * ** fv_list_def fresh list_sequent_def inst_def
+            using instt_def
+            by simp (frule calculation.intros(2),auto simp add: maps instt base frees,
+                metis (no_types,lifting) Suc_leD diff_Suc_Suc diff_diff_cancel diff_le_self
+                le_SucI list.map map_append snd_conv sound_Uni)
         next
           case notUni: False then show ?thesis
-            proof (cases "\<exists>a f list. t = (a,Exi f) # list")
-             case True
-              then obtain a and f and list where 1: "t = (a,Exi f) # list" by blast
-              then show ?thesis using IH assms * ** fresh list_sequent_def inst_def instt
+          proof (cases \<open>\<exists>a f list. t = (a,Exi f) # list\<close>)
+            case True
+            then obtain a and f and list where 1: \<open>t = (a,Exi f) # list\<close> by blast
+            then show ?thesis using IH assms * ** fresh list_sequent_def inst_def instt
               using instt_def
-                by simp (frule calculation.intros(2),simp,
-                   metis (no_types,lifting) Suc_leD diff_Suc_Suc diff_diff_cancel diff_le_self
-                    le_SucI list.map map_append snd_conv sound_Exi)
+              by simp (frule calculation.intros(2),simp,
+                  metis (no_types,lifting) Suc_leD diff_Suc_Suc diff_diff_cancel diff_le_self
+                  le_SucI list.map map_append snd_conv sound_Exi)
+          next
+            case notExi: False
+            then show ?thesis
+            proof (cases t)
+              case Nil
+              then show ?thesis using assms notAxiom IH * ** calculation_upwards
+                by (metis (no_types,lifting) calculation.intros(2) diff_Suc_Suc diff_diff_cancel
+                    diff_le_self list.set_intros(1) not_less_eq_eq solve.simps(1))
             next
-              case notExi: False
+              case (Cons a list)
               then show ?thesis
-              proof (cases t)
-                case Nil
-                then show ?thesis using assms notAxiom IH * ** calculation_upwards
-                   by (metis (no_types,lifting) calculation.intros(2) diff_Suc_Suc diff_diff_cancel
-                     diff_le_self list.set_intros(1) not_less_eq_eq solve.simps(1))
-              next
-                case (Cons a list)
-                then show ?thesis
                 using IH
-                proof (simp add: valid_def semantics_alternative_def2,intro allI impI)
-                  fix as gs g
-                  show "\<forall>n t. x = m - n \<and> (n,t) \<in> calculation s \<longrightarrow>
+              proof (simp add: valid_def semantics_alternative_def2,intro allI impI)
+                fix as gs g
+                show \<open>\<forall>n t. x = m - n \<and> (n,t) \<in> calculation s \<longrightarrow>
                        (\<forall>a b e. is_model_environment (a,b) e \<longrightarrow> (\<exists>p. p \<in> set (list_sequent t) \<and>
                          semantics (a,b) e p)) \<Longrightarrow>
                          is_model_environment (as,gs) g \<Longrightarrow> \<exists>p. p \<in> set (list_sequent (a # list))
-                         \<and> semantics (as,gs) g p"
-                  proof -
-                    assume ***: "is_model_environment (as,gs) g"
-                    and IH': "\<forall>n t. x = m - n \<and> (n,t) \<in> calculation s \<longrightarrow>
+                         \<and> semantics (as,gs) g p\<close>
+                proof -
+                  assume ***: \<open>is_model_environment (as,gs) g\<close>
+                    and IH': \<open>\<forall>n t. x = m - n \<and> (n,t) \<in> calculation s \<longrightarrow>
                                (\<forall>a b e. is_model_environment (a,b) e \<longrightarrow>
-                               (\<exists>p. p \<in> set (list_sequent t) \<and> semantics (a,b) e p))"
-                    then show ?thesis
-                    proof (cases a)
-                      case (Pair _ p) then show ?thesis
-                        proof (cases p)
-                          case (Pre b i v) then show ?thesis
-                            using IH' assms * ** Cons notAxiom *** Pair
-                            by (fastforce simp: list_sequent_def dest!: pre)
-                        next
-                          case (Con q r)
-                            then have 1: "(Suc n,list @ [(0,q)]) \<in> calculation s"
-                            using ** Pair con1 local.Cons notAxiom by blast
-                            then have 2: "x = m - Suc n \<and> (Suc n,list @ [(0,q)]) \<in> calculation s"
-                            using * by linarith
-                            have 3: "(Suc n,list @ [(0,r)]) \<in> calculation s"
-                            using ** Pair Con con2 local.Cons notAxiom by blast
-                            then have 4: "x = m - Suc n \<and> (Suc n,list @ [(0,r)]) \<in> calculation s"
-                            using * by linarith
-                            then have 5: "(Suc n,list @ [(0,q)]) \<in> calculation s \<longrightarrow>
+                               (\<exists>p. p \<in> set (list_sequent t) \<and> semantics (a,b) e p))\<close>
+                  then show ?thesis
+                  proof (cases a)
+                    case (Pair _ p) then show ?thesis
+                    proof (cases p)
+                      case (Pre b i v) then show ?thesis
+                        using IH' assms * ** Cons notAxiom *** Pair
+                        by (fastforce simp: list_sequent_def dest!: pre)
+                    next
+                      case (Con q r)
+                      then have 1: \<open>(Suc n,list @ [(0,q)]) \<in> calculation s\<close>
+                        using ** Pair con1 local.Cons notAxiom by blast
+                      then have 2: \<open>x = m - Suc n \<and> (Suc n,list @ [(0,q)]) \<in> calculation s\<close>
+                        using * by linarith
+                      have 3: \<open>(Suc n,list @ [(0,r)]) \<in> calculation s\<close>
+                        using ** Pair Con con2 local.Cons notAxiom by blast
+                      then have 4: \<open>x = m - Suc n \<and> (Suc n,list @ [(0,r)]) \<in> calculation s\<close>
+                        using * by linarith
+                      then have 5: \<open>(Suc n,list @ [(0,q)]) \<in> calculation s \<longrightarrow>
                               (\<forall>a b e. is_model_environment (a,b) e \<longrightarrow>
-                              (\<exists>p. p \<in> set (list_sequent (list @ [(0,q)])) \<and> semantics (a,b) e p))"
-                            using IH' by blast
-                            then have "x = m - Suc n \<and> (Suc n,list @ [(0,r)]) \<in> calculation s \<longrightarrow>
+                              (\<exists>p. p \<in> set (list_sequent (list @ [(0,q)])) \<and> semantics (a,b) e p))\<close>
+                        using IH' by blast
+                      then have \<open>x = m - Suc n \<and> (Suc n,list @ [(0,r)]) \<in> calculation s \<longrightarrow>
                             (\<forall>a b e. is_model_environment (a,b) e \<longrightarrow>
-                            (\<exists>p. p \<in> set (list_sequent (list @ [(0,r)])) \<and> semantics (a,b) e p))"
-                            using 2 IH' by blast
-                            then show ?thesis
-                            using 5
-                            proof (elim impE)
-                              show "(Suc n,list @ [(0,q)]) \<in> calculation s" using 1 by simp
-                            next
-                              show "\<forall>a b e. is_model_environment (a,b) e \<longrightarrow>
+                            (\<exists>p. p \<in> set (list_sequent (list @ [(0,r)])) \<and> semantics (a,b) e p))\<close>
+                        using 2 IH' by blast
+                      then show ?thesis
+                        using 5
+                      proof (elim impE)
+                        show \<open>(Suc n,list @ [(0,q)]) \<in> calculation s\<close> using 1 by simp
+                      next
+                        show \<open>\<forall>a b e. is_model_environment (a,b) e \<longrightarrow>
                                 (\<exists>p. p \<in> set (list_sequent (list @ [(0,q)])) \<and>
                                   semantics (a,b) e p) \<Longrightarrow>
-                                x = m - Suc n \<and> (Suc n,list @ [(0,r)]) \<in> calculation s"
-                              using 2 3 by blast
-                            next
-                              show "\<forall>a b e. is_model_environment (a,b) e \<longrightarrow>
+                                x = m - Suc n \<and> (Suc n,list @ [(0,r)]) \<in> calculation s\<close>
+                          using 2 3 by blast
+                      next
+                        show \<open>\<forall>a b e. is_model_environment (a,b) e \<longrightarrow>
                                 (\<exists>p. p \<in> set (list_sequent (list @ [(0,r)])) \<and>
                                   semantics (a,b) e p) \<Longrightarrow>
-                                 (Suc n,list @ [(0,q)]) \<in> calculation s"
-                              using 1 by blast
-                            next show "\<forall>a b e. is_model_environment (a,b) e \<longrightarrow>
+                                 (Suc n,list @ [(0,q)]) \<in> calculation s\<close>
+                          using 1 by blast
+                      next show \<open>\<forall>a b e. is_model_environment (a,b) e \<longrightarrow>
                               (\<exists>p. p \<in> set (list_sequent (list @ [(0,r)])) \<and> semantics (a,b) e p)
                               \<Longrightarrow> \<forall>a b e. is_model_environment (a,b) e \<longrightarrow>
                               (\<exists>p. p \<in> set (list_sequent (list @ [(0,q)])) \<and> semantics (a,b) e p)
-                              \<Longrightarrow> \<exists>p. p \<in> set (list_sequent (a # list)) \<and> semantics (as,gs) g p"
-                              using Con *** Pair list_sequent_def
-                              by simp (metis (no_types,lifting) semantics.simps(2))
-                            qed
-                      next
-                        case (Dis q r)
-                        then have "x = m - Suc n \<and> (Suc n,list @ [(0,q),(0,r)]) \<in> calculation s
+                              \<Longrightarrow> \<exists>p. p \<in> set (list_sequent (a # list)) \<and> semantics (as,gs) g p\<close>
+                          using Con *** Pair list_sequent_def
+                          by simp (metis (no_types,lifting) semantics.simps(2))
+                      qed
+                    next
+                      case (Dis q r)
+                      then have \<open>x = m - Suc n \<and> (Suc n,list @ [(0,q),(0,r)]) \<in> calculation s
                                   \<longrightarrow> (\<forall>a b e. is_model_environment (a,b) e \<longrightarrow>
                                   (\<exists>p. p \<in> set (list_sequent (list @ [(0,q),(0,r)])) \<and>
-                                  semantics (a,b) e p))"
-                                  using * IH' by blast
-                        then show ?thesis
-                        proof (elim impE)
-                          have 1: "(Suc n,list @ [(0,q),(0,r)]) \<in> calculation s"
-                            using ** Dis Pair dis local.Cons notAxiom by blast
-                          have "x = m - Suc n" using * by linarith
-                          then show "x = m - Suc n \<and> (Suc n,list @ [(0,q),(0,r)]) \<in> calculation s"
-                            using 1 by simp
-                        next
-                          show "\<forall>a b e. is_model_environment (a,b) e \<longrightarrow>
+                                  semantics (a,b) e p))\<close>
+                        using * IH' by blast
+                      then show ?thesis
+                      proof (elim impE)
+                        have 1: \<open>(Suc n,list @ [(0,q),(0,r)]) \<in> calculation s\<close>
+                          using ** Dis Pair dis local.Cons notAxiom by blast
+                        have \<open>x = m - Suc n\<close> using * by linarith
+                        then show \<open>x = m - Suc n \<and> (Suc n,list @ [(0,q),(0,r)]) \<in> calculation s\<close>
+                          using 1 by simp
+                      next
+                        show \<open>\<forall>a b e. is_model_environment (a,b) e \<longrightarrow>
                                (\<exists>p. p \<in> set (list_sequent (list @ [(0,q),(0,r)])) \<and>
                                  semantics (a,b) e p) \<Longrightarrow>
-                                 \<exists>p. p \<in> set (list_sequent (a # list)) \<and> semantics (as,gs) g p"
-                            using Dis *** Pair list_sequent_def
-                            by simp (metis (no_types,lifting) semantics.simps(3))
-                        qed
+                                 \<exists>p. p \<in> set (list_sequent (a # list)) \<and> semantics (as,gs) g p\<close>
+                          using Dis *** Pair list_sequent_def
+                          by simp (metis (no_types,lifting) semantics.simps(3))
+                      qed
                     next
                       case Uni then show ?thesis
                         using notUni Pair Cons by blast
@@ -1342,46 +1344,46 @@ next
   qed
 qed
 
-lemma list_make_sequent_inverse: "list_sequent (make_sequent s) = s"
-using list_sequent_def make_sequent_def
-by (induct s) simp_all
+lemma list_make_sequent_inverse: \<open>list_sequent (make_sequent s) = s\<close>
+  using list_sequent_def make_sequent_def
+  by (induct s) simp_all
 
 lemma soundness:
-  assumes "finite (calculation (make_sequent s))"
-  shows "valid s"
+  assumes \<open>finite (calculation (make_sequent s))\<close>
+  shows \<open>valid s\<close>
 proof -
-  have "init (make_sequent s)" and "finite (fst ` (calculation (make_sequent s)))"
+  have \<open>init (make_sequent s)\<close> and \<open>finite (fst ` (calculation (make_sequent s)))\<close>
     using assms by (simp add: init_def make_sequent_def,simp)
   then show ?thesis using assms soundness' list_make_sequent_inverse max_exists
     by (metis (mono_tags,lifting) empty_iff fst_conv image_eqI calculation.intros(1))
 qed
 
-subsection "Contains / Considers"
+subsection \<open>Contains / Considers\<close>
 
-definition contains :: "(nat \<Rightarrow> (nat \<times> sequent)) \<Rightarrow> nat \<Rightarrow> nat \<times> nnf \<Rightarrow> bool" where
-  "contains f n nf \<equiv> nf \<in> set (snd (f n))"
+definition contains :: \<open>(nat \<Rightarrow> (nat \<times> sequent)) \<Rightarrow> nat \<Rightarrow> nat \<times> nnf \<Rightarrow> bool\<close> where
+  \<open>contains f n nf \<equiv> nf \<in> set (snd (f n))\<close>
 
-definition considers :: "(nat \<Rightarrow> (nat \<times> sequent)) \<Rightarrow> nat \<Rightarrow> nat \<times> nnf \<Rightarrow> bool" where
-  "considers f n nf \<equiv> case snd (f n) of [] \<Rightarrow> False | (x # xs) \<Rightarrow> x = nf"
+definition considers :: \<open>(nat \<Rightarrow> (nat \<times> sequent)) \<Rightarrow> nat \<Rightarrow> nat \<times> nnf \<Rightarrow> bool\<close> where
+  \<open>considers f n nf \<equiv> case snd (f n) of [] \<Rightarrow> False | (x # xs) \<Rightarrow> x = nf\<close>
 
 lemma progress:
-  assumes "f = failing_path (calculation s)"
-  and "infinite (calculation s)"
-  shows "snd (f n) = a # l \<longrightarrow> (\<exists>zs'. snd (f (Suc n)) = l@zs')"
+  assumes \<open>f = failing_path (calculation s)\<close>
+    and \<open>infinite (calculation s)\<close>
+  shows \<open>snd (f n) = a # l \<longrightarrow> (\<exists>zs'. snd (f (Suc n)) = l@zs')\<close>
 proof -
-  obtain suc: "(snd (f (Suc n))) \<in> set (solve (snd (f n)))" using assms is_path_f by blast
+  obtain suc: \<open>(snd (f (Suc n))) \<in> set (solve (snd (f n)))\<close> using assms is_path_f by blast
   then show ?thesis
   proof (cases a)
     case (Pair _ p)
     then show ?thesis using suc
-    by (induct p,safe,simp_all add: stop split: if_splits) blast
+      by (induct p,safe,simp_all add: stop split: if_splits) blast
   qed
 qed
 
 lemma contains_considers':
-  assumes "f = failing_path (calculation s)"
-  and "infinite (calculation s)"
-  shows "\<forall>n ys. snd (f n) = xs@y # ys \<longrightarrow> (\<exists>m zs'. snd (f (n+m)) = y # zs')"
+  assumes \<open>f = failing_path (calculation s)\<close>
+    and \<open>infinite (calculation s)\<close>
+  shows \<open>\<forall>n ys. snd (f n) = xs@y # ys \<longrightarrow> (\<exists>m zs'. snd (f (n+m)) = y # zs')\<close>
 proof (induct xs)
   case Nil then show ?case using append.simps(1) by (metis Nat.add_0_right)
 next
@@ -1390,29 +1392,29 @@ next
 qed
 
 lemma contains_considers:
-  assumes "f = failing_path (calculation s)"
-  and "infinite (calculation s)"
-  and "contains f n y"
-  shows "(\<exists>m. considers f (n+m) y)"
-using assms
-by (clarsimp simp: contains_def considers_def dest!: split_list_first)
-  (frule contains_considers'[rule_format],simp,simp,metis (mono_tags,lifting) list.simps(5))
+  assumes \<open>f = failing_path (calculation s)\<close>
+    and \<open>infinite (calculation s)\<close>
+    and \<open>contains f n y\<close>
+  shows \<open>(\<exists>m. considers f (n+m) y)\<close>
+  using assms
+  by (clarsimp simp: contains_def considers_def dest!: split_list_first)
+    (frule contains_considers'[rule_format],simp,simp,metis (mono_tags,lifting) list.simps(5))
 
 lemma contains_propagates_Pre:
-  assumes "f = failing_path (calculation s)"
-  and "infinite (calculation s)"
-  and "contains f n (0,Pre b i v)"
-  shows "contains f (n+q) (0,Pre b i v)"
+  assumes \<open>f = failing_path (calculation s)\<close>
+    and \<open>infinite (calculation s)\<close>
+    and \<open>contains f n (0,Pre b i v)\<close>
+  shows \<open>contains f (n+q) (0,Pre b i v)\<close>
 proof (induct q)
   case 0 then show ?case using assms by simp
 next
   case IH: (Suc q')
-  then have "\<exists>ys zs. snd (f (n + q')) = ys @ (0,Pre b i v) # zs \<and> (0,Pre b i v) \<notin> set ys"
+  then have \<open>\<exists>ys zs. snd (f (n + q')) = ys @ (0,Pre b i v) # zs \<and> (0,Pre b i v) \<notin> set ys\<close>
     by (meson contains_def split_list_first)
   then obtain ys and zs where 1:
-    "snd (f (n + q')) = ys @ (0,Pre b i v) # zs \<and> (0,Pre b i v) \<notin> set ys"
+    \<open>snd (f (n + q')) = ys @ (0,Pre b i v) # zs \<and> (0,Pre b i v) \<notin> set ys\<close>
     by blast
-  then have 2: "(snd (f (Suc (n + q')))) \<in> set (solve (snd (f (n + q'))))"
+  then have 2: \<open>(snd (f (Suc (n + q')))) \<in> set (solve (snd (f (n + q'))))\<close>
     using assms is_path_f by blast
   then show ?case
   proof (cases ys)
@@ -1429,96 +1431,96 @@ next
 qed
 
 lemma contains_propagates_Con:
-  assumes "f = failing_path (calculation s)"
-  and "infinite (calculation s)"
-  and "contains f n (0,Con p q)"
-  shows "(\<exists>y. contains f (n+y) (0,p) \<or> contains f (n+y) (0,q))"
+  assumes \<open>f = failing_path (calculation s)\<close>
+    and \<open>infinite (calculation s)\<close>
+    and \<open>contains f n (0,Con p q)\<close>
+  shows \<open>(\<exists>y. contains f (n+y) (0,p) \<or> contains f (n+y) (0,q))\<close>
 proof -
-  have "(\<exists>l. considers f (n+l) (0,Con p q))" using assms contains_considers by blast
-  then obtain l where 1: "considers f (n+l) (0,Con p q)" by blast
-  then have 2: "(snd (f (Suc (n + l)))) \<in> set (solve (snd (f (n + l))))"
+  have \<open>(\<exists>l. considers f (n+l) (0,Con p q))\<close> using assms contains_considers by blast
+  then obtain l where 1: \<open>considers f (n+l) (0,Con p q)\<close> by blast
+  then have 2: \<open>(snd (f (Suc (n + l)))) \<in> set (solve (snd (f (n + l))))\<close>
     using assms is_path_f by blast
   then show ?thesis
-  proof (cases "snd (f (n + l))")
+  proof (cases \<open>snd (f (n + l))\<close>)
     case Nil then show ?thesis using 1 considers_def by simp
   next
     case Cons then show ?thesis using 1 2 considers_def contains_def
-      by (rule_tac x="Suc l" in exI) auto
+      by (rule_tac x=\<open>Suc l\<close> in exI) auto
   qed
 qed
 
 lemma contains_propagates_Dis:
-  assumes "f = failing_path (calculation s)"
-  and "infinite (calculation s)"
-  and "contains f n (0,Dis p q)"
-  shows "(\<exists>y. contains f (n+y) (0,p) \<and> contains f (n+y) (0,q))"
+  assumes \<open>f = failing_path (calculation s)\<close>
+    and \<open>infinite (calculation s)\<close>
+    and \<open>contains f n (0,Dis p q)\<close>
+  shows \<open>(\<exists>y. contains f (n+y) (0,p) \<and> contains f (n+y) (0,q))\<close>
 proof -
-  have "(\<exists>l. considers f (n+l) (0,Dis p q))" using assms contains_considers by blast
-  then obtain l where 1: "considers f (n+l) (0,Dis p q)" by blast
-  then have 2: "(snd (f (Suc (n + l)))) \<in> set (solve (snd (f (n + l))))"
+  have \<open>(\<exists>l. considers f (n+l) (0,Dis p q))\<close> using assms contains_considers by blast
+  then obtain l where 1: \<open>considers f (n+l) (0,Dis p q)\<close> by blast
+  then have 2: \<open>(snd (f (Suc (n + l)))) \<in> set (solve (snd (f (n + l))))\<close>
     using assms is_path_f by blast
   then show ?thesis
-  proof (cases "snd (f (n + l))")
+  proof (cases \<open>snd (f (n + l))\<close>)
     case Nil then show ?thesis using 1 considers_def by simp
   next
     case Cons then show ?thesis using 1 2 considers_def contains_def
-      by (rule_tac x="Suc l" in exI) simp_all
+      by (rule_tac x=\<open>Suc l\<close> in exI) simp_all
   qed
 qed
 
 lemma contains_propagates_Uni:
-  assumes "f = failing_path (calculation s)"
-  and "infinite (calculation s)"
-  and "contains f n (0,Uni p)"
-  shows "(\<exists>y. contains f (Suc(n+y)) (0,(sv (bind (fresh (fv_list (map snd (snd (f (n+y))))))) p)))"
+  assumes \<open>f = failing_path (calculation s)\<close>
+    and \<open>infinite (calculation s)\<close>
+    and \<open>contains f n (0,Uni p)\<close>
+  shows \<open>(\<exists>y. contains f (Suc(n+y)) (0,(sv (bind (fresh (fv_list (map snd (snd (f (n+y))))))) p)))\<close>
 proof -
-  have "(\<exists>l. considers f (n+l) (0,Uni p))" using assms contains_considers by blast
-  then obtain l where 1: "considers f (n+l) (0,Uni p)" by blast
-  then have 2: "(snd (f (Suc (n + l)))) \<in> set (solve (snd (f (n + l))))"
+  have \<open>(\<exists>l. considers f (n+l) (0,Uni p))\<close> using assms contains_considers by blast
+  then obtain l where 1: \<open>considers f (n+l) (0,Uni p)\<close> by blast
+  then have 2: \<open>(snd (f (Suc (n + l)))) \<in> set (solve (snd (f (n + l))))\<close>
     using assms is_path_f by blast
   then show ?thesis
-  proof (cases "snd (f (n + l))")
+  proof (cases \<open>snd (f (n + l))\<close>)
     case Nil then show ?thesis using 1 considers_def by simp
   next
     case Cons then show ?thesis
       using 1 2 considers_def contains_def inst_def instt base frees instt_def
-      by (rule_tac x="l" in exI) (simp add: fv_list_def maps_def)
+      by (rule_tac x=\<open>l\<close> in exI) (simp add: fv_list_def maps_def)
   qed
 qed
 
 lemma contains_propagates_Exi:
-  assumes "f = failing_path (calculation s)"
-  and "infinite (calculation s)"
-  and "contains f n (m,Exi p)"
-  shows "(\<exists>y. (contains f (n+y) (0,(sv (bind m) p)) \<and> (contains f (n+y) (Suc m,Exi p))))"
+  assumes \<open>f = failing_path (calculation s)\<close>
+    and \<open>infinite (calculation s)\<close>
+    and \<open>contains f n (m,Exi p)\<close>
+  shows \<open>(\<exists>y. (contains f (n+y) (0,(sv (bind m) p)) \<and> (contains f (n+y) (Suc m,Exi p))))\<close>
 proof -
-  have "(\<exists>l. considers f (n+l) (m,Exi p))" using assms contains_considers by blast
-  then obtain l where 1: "considers f (n+l) (m,Exi p)" by blast
-  then have 2: "(snd (f (Suc (n + l)))) \<in> set (solve (snd (f (n + l))))"
+  have \<open>(\<exists>l. considers f (n+l) (m,Exi p))\<close> using assms contains_considers by blast
+  then obtain l where 1: \<open>considers f (n+l) (m,Exi p)\<close> by blast
+  then have 2: \<open>(snd (f (Suc (n + l)))) \<in> set (solve (snd (f (n + l))))\<close>
     using assms is_path_f by blast
   then show ?thesis
-  proof (cases "snd (f (n + l))")
+  proof (cases \<open>snd (f (n + l))\<close>)
     case Nil then show ?thesis using 1 considers_def by simp
   next
     case Cons then show ?thesis using 1 2 considers_def contains_def inst_def
-      using instt instt_def by (rule_tac x="Suc l" in exI) simp
+      using instt instt_def by (rule_tac x=\<open>Suc l\<close> in exI) simp
   qed
 qed
 
 lemma Exi_downward:
-  assumes "f = failing_path (calculation s)"
-  and "infinite (calculation s)"
-  and "init s"
-  shows "\<forall>m. (Suc m,Exi g) \<in> set (snd (f n)) \<longrightarrow> (\<exists>n'. (m,Exi g) \<in> set (snd (f n')))"
+  assumes \<open>f = failing_path (calculation s)\<close>
+    and \<open>infinite (calculation s)\<close>
+    and \<open>init s\<close>
+  shows \<open>\<forall>m. (Suc m,Exi g) \<in> set (snd (f n)) \<longrightarrow> (\<exists>n'. (m,Exi g) \<in> set (snd (f n')))\<close>
 proof (induct n)
   case 0 then show ?case using assms init_def is_path_f_0 by fastforce
 next
   case IH: (Suc x)
-  then have fxSuc: "f x \<in> calculation s \<and> fst (f x) = x \<and>
-    snd (f (Suc x)) \<in> set (solve (snd (f x))) \<and> infinite (calculation (snd (f x)))"
+  then have fxSuc: \<open>f x \<in> calculation s \<and> fst (f x) = x \<and>
+    snd (f (Suc x)) \<in> set (solve (snd (f x))) \<and> infinite (calculation (snd (f x)))\<close>
     using assms is_path_f by blast
   then show ?case
-  proof (cases "f x")
+  proof (cases \<open>f x\<close>)
     case fxPair: (Pair _ l)
     then show ?thesis
     proof (cases l)
@@ -1549,88 +1551,88 @@ next
 qed
 
 lemma Exi0:
-  assumes "f = failing_path (calculation s)"
-  and "infinite (calculation s)"
-  and "init s"
-  shows "\<forall>n. contains f n (m,Exi g) \<longrightarrow> (\<exists>n'. contains f n' (0,Exi g))"
-using assms Exi_downward contains_def
-by (induct m) auto
+  assumes \<open>f = failing_path (calculation s)\<close>
+    and \<open>infinite (calculation s)\<close>
+    and \<open>init s\<close>
+  shows \<open>\<forall>n. contains f n (m,Exi g) \<longrightarrow> (\<exists>n'. contains f n' (0,Exi g))\<close>
+  using assms Exi_downward contains_def
+  by (induct m) auto
 
 lemma Exi_upward':
-  assumes "f = failing_path (calculation s)"
-  and "infinite (calculation s)"
-  and "init s"
-  shows "\<forall>n. contains f n (0,Exi g) \<longrightarrow> (\<exists>n'. contains f n' (m,Exi g))"
-using assms contains_propagates_Exi
-by (induct m) (simp,blast)
+  assumes \<open>f = failing_path (calculation s)\<close>
+    and \<open>infinite (calculation s)\<close>
+    and \<open>init s\<close>
+  shows \<open>\<forall>n. contains f n (0,Exi g) \<longrightarrow> (\<exists>n'. contains f n' (m,Exi g))\<close>
+  using assms contains_propagates_Exi
+  by (induct m) (simp,blast)
 
 lemma Exi_upward:
-  assumes "f = failing_path (calculation s)"
-  and "infinite (calculation s)"
-  and "init s"
-  and "contains f n (m,Exi g)"
-  shows "(\<forall>m'. \<exists>n'. contains f n' (0,sv (bind m') g))"
+  assumes \<open>f = failing_path (calculation s)\<close>
+    and \<open>infinite (calculation s)\<close>
+    and \<open>init s\<close>
+    and \<open>contains f n (m,Exi g)\<close>
+  shows \<open>(\<forall>m'. \<exists>n'. contains f n' (0,sv (bind m') g))\<close>
 proof -
   fix m'
-  have "\<exists>n'. contains f n' (m',Exi g)" using assms Exi0 Exi_upward' by metis
+  have \<open>\<exists>n'. contains f n' (m',Exi g)\<close> using assms Exi0 Exi_upward' by metis
   then show ?thesis using assms contains_propagates_Exi Exi0 Exi_upward' by metis
 qed
 
-definition ntou :: "nat \<Rightarrow> proxy" where
-  "ntou n \<equiv> replicate n ()"
+definition ntou :: \<open>nat \<Rightarrow> proxy\<close> where
+  \<open>ntou n \<equiv> replicate n ()\<close>
 
-definition uton :: "proxy \<Rightarrow> nat" where
-  "uton u \<equiv> length u"
+definition uton :: \<open>proxy \<Rightarrow> nat\<close> where
+  \<open>uton u \<equiv> length u\<close>
 
-lemma ntou_uton: "ntou (uton u) = u"
-using ntou_def uton_def
-by (induct u) auto
+lemma ntou_uton: \<open>ntou (uton u) = u\<close>
+  using ntou_def uton_def
+  by (induct u) auto
 
-lemma uton_ntou: "uton (ntou n) = n"
-using ntou_def uton_def
-by (induct n) auto
+lemma uton_ntou: \<open>uton (ntou n) = n\<close>
+  using ntou_def uton_def
+  by (induct n) auto
 
-lemma uton_ntou_id: "uton \<circ> ntou = id"
-using uton_ntou by auto
+lemma uton_ntou_id: \<open>uton \<circ> ntou = id\<close>
+  using uton_ntou by auto
 
-subsection "Falsifying Model From Failing Path"
+subsection \<open>Falsifying Model From Failing Path\<close>
 
-definition model :: "sequent \<Rightarrow> model" where
-  "model s \<equiv> (range ntou,\<lambda> p ms. (let f = failing_path (calculation s) in
-    (\<forall>n m. \<not> contains f n (m,Pre True p (map uton ms)))))"
+definition model :: \<open>sequent \<Rightarrow> model\<close> where
+  \<open>model s \<equiv> (range ntou,\<lambda> p ms. (let f = failing_path (calculation s) in
+    (\<forall>n m. \<not> contains f n (m,Pre True p (map uton ms)))))\<close>
 
-lemma is_env_model_ntou: "is_model_environment (model s) ntou"
-using is_model_environment_def model_def
-by simp
+lemma is_env_model_ntou: \<open>is_model_environment (model s) ntou\<close>
+  using is_model_environment_def model_def
+  by simp
 
 lemma not_is_Exi:
-  assumes "f = failing_path (calculation s)"
-  and "infinite (calculation s)"
-  and "init s"
-  and "(contains f n (m,p))"
-  shows "\<not> is_Exi p \<Longrightarrow> m = 0"
-using assms contains_def index0 is_path_f' prod.collapse
-by metis
+  assumes \<open>f = failing_path (calculation s)\<close>
+    and \<open>infinite (calculation s)\<close>
+    and \<open>init s\<close>
+    and \<open>(contains f n (m,p))\<close>
+  shows \<open>\<not> is_Exi p \<Longrightarrow> m = 0\<close>
+  using assms contains_def index0 is_path_f' prod.collapse
+  by metis
 
-lemma size_subst: "size (sv f p) = size p"
-by (induct p arbitrary: f) simp_all
+lemma size_subst: \<open>size (sv f p) = size p\<close>
+  by (induct p arbitrary: f) simp_all
 
-lemma size_bind: "size (sv (bind m) p) = size p"
-using bind_def size_subst
-by simp
+lemma size_bind: \<open>size (sv (bind m) p) = size p\<close>
+  using bind_def size_subst
+  by simp
 
 lemma model':
-  assumes "f = failing_path (calculation s)"
-  and "infinite (calculation s)"
-  and "init s"
-  shows "\<forall>p. size p = h \<longrightarrow> (\<forall>m n. contains f n (m,p) \<longrightarrow> \<not> (semantics (model s) ntou p))"
+  assumes \<open>f = failing_path (calculation s)\<close>
+    and \<open>infinite (calculation s)\<close>
+    and \<open>init s\<close>
+  shows \<open>\<forall>p. size p = h \<longrightarrow> (\<forall>m n. contains f n (m,p) \<longrightarrow> \<not> (semantics (model s) ntou p))\<close>
 proof (rule nat_less_induct,rule allI)
   fix p n
-  show "\<forall>m<n. \<forall>p. size p = m \<longrightarrow> (\<forall>m n. contains f n (m,p) \<longrightarrow> \<not> semantics (model s) ntou p) \<Longrightarrow>
-    size p = n \<longrightarrow> (\<forall>m n. contains f n (m,p) \<longrightarrow> \<not> semantics (model s) ntou p)"
+  show \<open>\<forall>m<n. \<forall>p. size p = m \<longrightarrow> (\<forall>m n. contains f n (m,p) \<longrightarrow> \<not> semantics (model s) ntou p) \<Longrightarrow>
+    size p = n \<longrightarrow> (\<forall>m n. contains f n (m,p) \<longrightarrow> \<not> semantics (model s) ntou p)\<close>
   proof -
-    assume *: "\<forall>m<n. \<forall>p. size p = m \<longrightarrow> (\<forall>m n. contains f n (m,p) \<longrightarrow>
-      \<not> semantics (model s) ntou p)"
+    assume *: \<open>\<forall>m<n. \<forall>p. size p = m \<longrightarrow> (\<forall>m n. contains f n (m,p) \<longrightarrow>
+      \<not> semantics (model s) ntou p)\<close>
     show ?thesis
     proof (cases p)
       case (Pre b i v) then show ?thesis
@@ -1640,23 +1642,23 @@ proof (rule nat_less_induct,rule allI)
         case False then show ?thesis using Pre
         proof (clarsimp simp: model_def uton_ntou_id)
           fix na m nb ma
-          show "n = 0 \<Longrightarrow> contains f na (m,Pre False i v) \<Longrightarrow>
-            contains (failing_path (calculation s)) nb (ma,Pre True i v) \<Longrightarrow> False"
+          show \<open>n = 0 \<Longrightarrow> contains f na (m,Pre False i v) \<Longrightarrow>
+            contains (failing_path (calculation s)) nb (ma,Pre True i v) \<Longrightarrow> False\<close>
           proof -
-            assume 1: "contains f na (m,Pre False i v)" and
-                   2: "contains (failing_path (calculation s)) nb (ma,Pre True i v)"
-            then have 3: "m = 0 \<and> ma = 0" using assms is_Exi not_is_Exi by simp
-            then have "\<exists>y. considers (failing_path (calculation s)) (nb+na+y) (0,Pre True i v)"
-            using assms 2 contains_considers contains_propagates_Pre by simp
+            assume 1: \<open>contains f na (m,Pre False i v)\<close> and
+              2: \<open>contains (failing_path (calculation s)) nb (ma,Pre True i v)\<close>
+            then have 3: \<open>m = 0 \<and> ma = 0\<close> using assms is_Exi not_is_Exi by simp
+            then have \<open>\<exists>y. considers (failing_path (calculation s)) (nb+na+y) (0,Pre True i v)\<close>
+              using assms 2 contains_considers contains_propagates_Pre by simp
             then obtain y
-            where 4: "considers (failing_path (calculation s)) (nb+na+y) (0,Pre True i v)"
-            by blast
-            then have 5: "contains (failing_path (calculation s)) (na+nb+y) (0,Pre False i v)"
-            using assms 1 3 contains_propagates_Pre by simp
-            then have 6: "nb+na=na+nb"
-            by simp
-            then have "is_axiom (list_sequent (snd ((failing_path (calculation s)) (na+nb+y))))"
-            proof (cases "snd ((failing_path (calculation s)) (na + nb + y))")
+              where 4: \<open>considers (failing_path (calculation s)) (nb+na+y) (0,Pre True i v)\<close>
+              by blast
+            then have 5: \<open>contains (failing_path (calculation s)) (na+nb+y) (0,Pre False i v)\<close>
+              using assms 1 3 contains_propagates_Pre by simp
+            then have 6: \<open>nb+na=na+nb\<close>
+              by simp
+            then have \<open>is_axiom (list_sequent (snd ((failing_path (calculation s)) (na+nb+y))))\<close>
+            proof (cases \<open>snd ((failing_path (calculation s)) (na + nb + y))\<close>)
               case Nil then show ?thesis using 5 contains_def by simp
             next
               case Cons then show ?thesis
@@ -1669,35 +1671,35 @@ proof (rule nat_less_induct,rule allI)
     next
       case Con then show ?thesis using assms * is_Exi not_is_Exi contains_propagates_Con
         by (metis Nat.add_0_right add_Suc_right nnf.size(7)
-          less_add_Suc1 less_add_Suc2 semantics.simps(2))
+            less_add_Suc1 less_add_Suc2 semantics.simps(2))
     next
       case Dis then show ?thesis using assms * contains_propagates_Dis is_Exi not_is_Exi
         by (metis Nat.add_0_right add_Suc_right nnf.size(8)
-              less_add_Suc1 less_add_Suc2 semantics.simps(3))
+            less_add_Suc1 less_add_Suc2 semantics.simps(3))
     next
       case (Uni q) then show ?thesis
       proof (intro impI allI)
         fix na m
-        show "size p = n \<Longrightarrow> contains f na (m,p) \<Longrightarrow> \<not> semantics (model s) ntou p"
+        show \<open>size p = n \<Longrightarrow> contains f na (m,p) \<Longrightarrow> \<not> semantics (model s) ntou p\<close>
         proof -
-          assume 1: "size p = n" and 2: "contains f na (m,p)"
-          then have "m = 0" using assms Uni is_Exi not_is_Exi by simp
-          then have "\<exists>y. contains f (Suc (na + y)) (0,(sv (bind (fresh (fv_list
-            (map snd (snd (f (na + y))))))) q))"
+          assume 1: \<open>size p = n\<close> and 2: \<open>contains f na (m,p)\<close>
+          then have \<open>m = 0\<close> using assms Uni is_Exi not_is_Exi by simp
+          then have \<open>\<exists>y. contains f (Suc (na + y)) (0,(sv (bind (fresh (fv_list
+              (map snd (snd (f (na + y))))))) q))\<close>
             using assms Uni 2 contains_propagates_Uni by simp
-          then obtain y where 3: "contains f (Suc (na + y)) (0,sv (bind (fresh (fv_list
-            (map snd (snd (f (na + y))))))) q)"
+          then obtain y where 3: \<open>contains f (Suc (na + y)) (0,sv (bind (fresh (fv_list
+              (map snd (snd (f (na + y))))))) q)\<close>
             by blast
-          have 4: "Suc (size q) = n" using Uni 1 by simp
+          have 4: \<open>Suc (size q) = n\<close> using Uni 1 by simp
           then show ?thesis using Uni
           proof (simp)
-            show "\<exists>z\<in>fst (model s). \<not> semantics (model s) (case_nat z ntou) q"
-            proof (rule_tac x="ntou (fresh (fv_list (map snd (snd (f (na + y))))))" in bexI)
-              show "\<not> semantics (model s) (case_nat (ntou (fresh (fv_list
-                (map snd (snd (f (na + y))))))) ntou) q"
-              using * 3 4 eval_bind size_bind lessI by metis
+            show \<open>\<exists>z\<in>fst (model s). \<not> semantics (model s) (case_nat z ntou) q\<close>
+            proof (rule_tac x=\<open>ntou (fresh (fv_list (map snd (snd (f (na + y))))))\<close> in bexI)
+              show \<open>\<not> semantics (model s) (case_nat (ntou (fresh (fv_list
+                  (map snd (snd (f (na + y))))))) ntou) q\<close>
+                using * 3 4 eval_bind size_bind lessI by metis
             next
-              show "ntou (fresh (fv_list (map snd (snd (f (na + y)))))) \<in> fst (model s)"
+              show \<open>ntou (fresh (fv_list (map snd (snd (f (na + y)))))) \<in> fst (model s)\<close>
                 using is_env_model_ntou is_model_environment_def by blast
             qed
           qed
@@ -1707,14 +1709,14 @@ proof (rule nat_less_induct,rule allI)
       case (Exi q) then show ?thesis
       proof (clarsimp)
         fix m na ma z
-        show "p = Exi q \<Longrightarrow> n = Suc (size q) \<Longrightarrow> z \<in> fst (model s) \<Longrightarrow> contains f na (m,Exi q)
-          \<Longrightarrow> semantics (model s) (case_nat z ntou) q \<Longrightarrow> False"
+        show \<open>p = Exi q \<Longrightarrow> n = Suc (size q) \<Longrightarrow> z \<in> fst (model s) \<Longrightarrow> contains f na (m,Exi q)
+            \<Longrightarrow> semantics (model s) (case_nat z ntou) q \<Longrightarrow> False\<close>
         proof -
-          assume "n = Suc (size q)" and "contains f na (m,Exi q)"
-          and 1: "semantics (model s) (case_nat z ntou) q"
-          then have "\<forall>m'. \<not> semantics (model s) ntou (sv (bind m') q)"
+          assume \<open>n = Suc (size q)\<close> and \<open>contains f na (m,Exi q)\<close>
+            and 1: \<open>semantics (model s) (case_nat z ntou) q\<close>
+          then have \<open>\<forall>m'. \<not> semantics (model s) ntou (sv (bind m') q)\<close>
             using assms * by (meson Exi_upward eval_cong id_apply lessI size_bind)
-          also have "\<forall>u. ntou (uton u) = u" using ntou_uton by simp
+          also have \<open>\<forall>u. ntou (uton u) = u\<close> using ntou_uton by simp
           ultimately show ?thesis using 1 eval_bind by metis
         qed
       qed
@@ -1723,120 +1725,120 @@ proof (rule nat_less_induct,rule allI)
 qed
 
 lemma model:
-  assumes "f = failing_path (calculation s)"
-  and "infinite (calculation s)"
-  and "init s"
-  shows "(\<forall>p m n. contains f n (m,p) \<longrightarrow> \<not> (semantics (model s) ntou p))"
-using assms model'
-by simp
+  assumes \<open>f = failing_path (calculation s)\<close>
+    and \<open>infinite (calculation s)\<close>
+    and \<open>init s\<close>
+  shows \<open>(\<forall>p m n. contains f n (m,p) \<longrightarrow> \<not> (semantics (model s) ntou p))\<close>
+  using assms model'
+  by simp
 
-subsection "Completeness"
+subsection \<open>Completeness\<close>
 
-lemma completeness': "infinite (calculation s) \<Longrightarrow> init s \<Longrightarrow>
-    \<forall>mA \<in> set s. \<not> semantics (model s) ntou (snd mA)"
-by (metis contains_def eq_snd_iff is_path_f_0 model)
+lemma completeness': \<open>infinite (calculation s) \<Longrightarrow> init s \<Longrightarrow>
+    \<forall>mA \<in> set s. \<not> semantics (model s) ntou (snd mA)\<close>
+  by (metis contains_def eq_snd_iff is_path_f_0 model)
 
-lemma completeness'': "infinite (calculation (make_sequent s)) \<Longrightarrow>
-    init (make_sequent s) \<Longrightarrow> \<forall>p. p \<in> set s \<longrightarrow> \<not> semantics (model (make_sequent s)) ntou p"
-using completeness' make_sequent_def
-by fastforce
+lemma completeness'': \<open>infinite (calculation (make_sequent s)) \<Longrightarrow>
+    init (make_sequent s) \<Longrightarrow> \<forall>p. p \<in> set s \<longrightarrow> \<not> semantics (model (make_sequent s)) ntou p\<close>
+  using completeness' make_sequent_def
+  by fastforce
 
-lemma completeness: "infinite (calculation (make_sequent s)) \<Longrightarrow> \<not> valid s"
-using valid_def init_def make_sequent_def is_env_model_ntou semantics_alternative_def2
-  completeness''
-by (subgoal_tac "init (make_sequent s)") (metis,simp)
+lemma completeness: \<open>infinite (calculation (make_sequent s)) \<Longrightarrow> \<not> valid s\<close>
+  using valid_def init_def make_sequent_def is_env_model_ntou semantics_alternative_def2
+    completeness''
+  by (subgoal_tac \<open>init (make_sequent s)\<close>) (metis,simp)
 
-subsection "Algorithm"
+subsection \<open>Algorithm\<close>
 
-definition loop :: "sequent list \<Rightarrow> nat \<Rightarrow> sequent list" where
-  "loop s n \<equiv> repeat' (concat \<circ> map solve) s n"
+definition loop :: \<open>sequent list \<Rightarrow> nat \<Rightarrow> sequent list\<close> where
+  \<open>loop s n \<equiv> repeat' (concat \<circ> map solve) s n\<close>
 
-lemma loop_upwards: "loop s n = [] \<Longrightarrow> loop s (n+m) = []"
-using loop_def
-by (induct m) auto
+lemma loop_upwards: \<open>loop s n = [] \<Longrightarrow> loop s (n+m) = []\<close>
+  using loop_def
+  by (induct m) auto
 
-lemma concat_append: "concat (xs@ys) = ((concat xs) @ (concat ys))"
-by (induct xs) auto
+lemma concat_append: \<open>concat (xs@ys) = ((concat xs) @ (concat ys))\<close>
+  by (induct xs) auto
 
-lemma set_concat: "set (concat xs) = \<Union> (set ` set xs)"
-by (induct xs) auto
+lemma set_concat: \<open>set (concat xs) = \<Union> (set ` set xs)\<close>
+  by (induct xs) auto
 
-lemma loop: "\<forall>x. ((n,x) \<in> calculation s) = (x \<in> set (loop [s] n))"
+lemma loop: \<open>\<forall>x. ((n,x) \<in> calculation s) = (x \<in> set (loop [s] n))\<close>
 proof (induct n)
   case 0 then show ?case using loop_def calculation_init by simp
 next
   case (Suc m) then show ?case
   proof (intro allI iffI)
     fix x ys z
-    assume "(Suc m,x) \<in> calculation s"
-    then have "\<exists>t. (m,t) \<in> calculation s \<and> x \<in> set (solve t) \<and> \<not> is_axiom (list_sequent t)"
+    assume \<open>(Suc m,x) \<in> calculation s\<close>
+    then have \<open>\<exists>t. (m,t) \<in> calculation s \<and> x \<in> set (solve t) \<and> \<not> is_axiom (list_sequent t)\<close>
       using calculation_downwards by blast
     then obtain t
-      where 1: "(m,t) \<in> calculation s \<and> x \<in> set (solve t) \<and> \<not> is_axiom (list_sequent t)"
+      where 1: \<open>(m,t) \<in> calculation s \<and> x \<in> set (solve t) \<and> \<not> is_axiom (list_sequent t)\<close>
       by blast
-      then show "(x \<in> set (loop [s] (Suc m)))"
-        using Suc loop_def by (clarsimp dest!: split_list_first)
+    then show \<open>(x \<in> set (loop [s] (Suc m)))\<close>
+      using Suc loop_def by (clarsimp dest!: split_list_first)
   next
     fix x
-    assume "(x \<in> set (loop [s] (Suc m)))"
-    then show "(Suc m,x) \<in> calculation s"
+    assume \<open>(x \<in> set (loop [s] (Suc m)))\<close>
+    then show \<open>(Suc m,x) \<in> calculation s\<close>
       using Suc by (fastforce simp: set_concat loop_def calculation.intros(2))
   qed
 qed
 
-lemma calculation_f: "calculation s = UNION UNIV (\<lambda>x. set (map (\<lambda>y. (x,y)) (loop [s] x)))"
-using loop
-by fastforce
+lemma calculation_f: \<open>calculation s = UNION UNIV (\<lambda>x. set (map (\<lambda>y. (x,y)) (loop [s] x)))\<close>
+  using loop
+  by fastforce
 
 lemma finite_calculation':
-  assumes "finite (calculation s)"
-  shows "(\<exists>m. loop [s] m = [])"
+  assumes \<open>finite (calculation s)\<close>
+  shows \<open>(\<exists>m. loop [s] m = [])\<close>
 proof -
-  have "finite (fst ` (calculation s))" using assms by simp
-  then obtain x where xMax: "x \<in> fst ` calculation s \<and> (\<forall>y. y \<in> fst ` calculation s \<longrightarrow> y \<le> x)"
+  have \<open>finite (fst ` (calculation s))\<close> using assms by simp
+  then obtain x where xMax: \<open>x \<in> fst ` calculation s \<and> (\<forall>y. y \<in> fst ` calculation s \<longrightarrow> y \<le> x)\<close>
     using max_exists calculation.simps by (metis empty_iff image_is_empty)
   then show ?thesis
-  proof (cases "loop [s] (Suc x)")
-    assume "loop [s] (Suc x) = []" then show ?thesis by blast
+  proof (cases \<open>loop [s] (Suc x)\<close>)
+    assume \<open>loop [s] (Suc x) = []\<close> then show ?thesis by blast
   next
     fix a l
-    assume "loop [s] (Suc x) = a # l"
-    then have "(Suc x,a) \<in> calculation s" using loop by simp
+    assume \<open>loop [s] (Suc x) = a # l\<close>
+    then have \<open>(Suc x,a) \<in> calculation s\<close> using loop by simp
     then show ?thesis using xMax by fastforce
   qed
 qed
 
 lemma finite_calculation'':
-  assumes "(\<exists>m. loop [s] m = [])"
-  shows "finite (calculation s)"
+  assumes \<open>(\<exists>m. loop [s] m = [])\<close>
+  shows \<open>finite (calculation s)\<close>
 proof -
-  obtain m where "loop [s] m = []" using assms by blast
-  then have "\<forall>y. loop [s] (m+y) = []" using loop_upwards by simp
-  then have 1: "(UN x:Collect (op \<le> m). Pair x ` set (loop [s] x)) = (UN x:Collect (op \<le> m). {})"
+  obtain m where \<open>loop [s] m = []\<close> using assms by blast
+  then have \<open>\<forall>y. loop [s] (m+y) = []\<close> using loop_upwards by simp
+  then have 1: \<open>(UN x:Collect (op \<le> m). Pair x ` set (loop [s] x)) = (UN x:Collect (op \<le> m). {})\<close>
     using SUP_cong image_is_empty le_Suc_ex mem_Collect_eq set_empty
-      by (metis (no_types,lifting))
-    then have "(UNIV::nat set) = {y. y < m} Un {y. m \<le> y}" by fastforce
-    then show ?thesis using 1 calculation_f by (clarsimp elim!: ssubst)
+    by (metis (no_types,lifting))
+  then have \<open>(UNIV::nat set) = {y. y < m} Un {y. m \<le> y}\<close> by fastforce
+  then show ?thesis using 1 calculation_f by (clarsimp elim!: ssubst)
 qed
 
-lemma finite_calculation: "finite (calculation s) = (\<exists>m. loop [s] m = [])"
-using finite_calculation' finite_calculation''
-by blast
+lemma finite_calculation: \<open>finite (calculation s) = (\<exists>m. loop [s] m = [])\<close>
+  using finite_calculation' finite_calculation''
+  by blast
 
-corollary finite_calculation_prover': "finite (calculation s) = iterator null (maps solve) [s]"
-using finite_calculation loop_def iterator_def maps null.simps list.exhaust rr
-by metis
+corollary finite_calculation_prover': \<open>finite (calculation s) = iterator null (maps solve) [s]\<close>
+  using finite_calculation loop_def iterator_def maps null.simps list.exhaust rr
+  by metis
 
-corollary finite_calculation_prover: "finite (calculation s) = iterator null solves [s]"
-using finite_calculation_prover' ms by simp
+corollary finite_calculation_prover: \<open>finite (calculation s) = iterator null solves [s]\<close>
+  using finite_calculation_prover' ms by simp
 
-section "Correctness"
+section \<open>Correctness\<close>
 
 lemmas magic = soundness completeness finite_calculation_prover
 
 theorem correctness: CHECK VALID
 proof -
-  have "\<forall>p. [[(0,p)]] = [map (Pair 0) [p]]" by simp
+  have \<open>\<forall>p. [[(0,p)]] = [map (Pair 0) [p]]\<close> by simp
   then have CHECK
     unfolding check_def
     using magic valid_def make_sequent_def semantics_alternative.simps main_def
@@ -1846,51 +1848,51 @@ proof -
   ultimately show CHECK VALID .
 qed
 
-corollary "\<exists>p. check p" "\<exists>p. \<not> check p"
+corollary \<open>\<exists>p. check p\<close> \<open>\<exists>p. \<not> check p\<close>
 proof -
-  have "\<not> valid [Pre True 0 []]" "valid [Dis (Pre True 0 []) (Pre False 0 [])]"
+  have \<open>\<not> valid [Pre True 0 []]\<close> \<open>valid [Dis (Pre True 0 []) (Pre False 0 [])]\<close>
     using valid_def is_model_environment_def by auto
-  then show "\<exists>p. check p" "\<exists>p. \<not> check p"
+  then show \<open>\<exists>p. check p\<close> \<open>\<exists>p. \<not> check p\<close>
     using magic correctness semantics_alternative.simps valid_def by (metis,metis)
 qed
 
-section "Code Generation"
+section \<open>Code Generation\<close>
 
-value "check test"
+value \<open>check test\<close>
 
-value "check (Dis (Pre True 0 []) (Pre False 0 []))"
+value \<open>check (Dis (Pre True 0 []) (Pre False 0 []))\<close>
 
-(* value "check (Pre True 0 [])" *)
+(* value \<open>check (Pre True 0 [])\<close> *)
 
-proposition "check test"
-by eval
+proposition \<open>check test\<close>
+  by eval
 
-proposition "check (Dis (Pre True 0 []) (Pre False 0 []))"
-by eval
+proposition \<open>check (Dis (Pre True 0 []) (Pre False 0 []))\<close>
+  by eval
 
-proposition "check test"
-by normalization
+proposition \<open>check test\<close>
+  by normalization
 
-proposition "check (Dis (Pre b i v) (Pre (\<not> b) i v))"
-by normalization
+proposition \<open>check (Dis (Pre b i v) (Pre (\<not> b) i v))\<close>
+  by normalization
 
 code_reflect X datatypes nnf = _ and nat = _ functions check
 
 ML_val
 
-{*
+\<open>
 
 val true = X.check (X.Dis (X.Uni (X.Con (X.Pre (false,X.Zero_nat,[X.Zero_nat]),
                                          X.Pre (false,X.Suc X.Zero_nat,[X.Zero_nat]))),
                            X.Dis (X.Exi (X.Pre (true,X.Suc X.Zero_nat,[X.Zero_nat])),
                                   X.Exi (X.Pre (true,X.Zero_nat,[X.Zero_nat])))))
 
-*}
+\<close>
 
 export_code check test in SML module_name X
 
-section "Acknowledgements"
+section \<open>Acknowledgements\<close>
 
-text "Based on the Archive of Formal Proofs entry Verified_Prover by Tom Ridge (TPHOLs 2005)"
+text \<open>Based on the Archive of Formal Proofs entry Verified_Prover by Tom Ridge (TPHOLs 2005)\<close>
 
 end
